intermediate before extending represents

erasure/theories/EWcbvEvalNamed.v
@@ -35,7 +35,7 @@ Inductive value : Set :=
 
 Definition environment := list (ident * value).
 Definition add : ident -> value -> environment -> environment := fun (x : ident) (v : value) env =>
-   (x, v) :: env.
+                                                                (x, v) :: env.
 Fixpoint add_multiple (xs : list ident) (vs : list value) (env : environment) : environment := 
   match xs, vs with
   | x :: xs, v :: vs => add x v (add_multiple xs vs env)
@@ -50,10 +50,10 @@ Definition lookup (E : environment) x :=
 
 Definition fix_env (l : list (ident * term)) Γ :=
   let fix aux (n : nat) : list value :=
-      match n with
-      | 0 => []
-      | S n0 => vRecClos l n0 Γ :: aux n0
-      end in
+    match n with
+    | 0 => []
+    | S n0 => vRecClos l n0 Γ :: aux n0
+    end in
   aux #|l|.
 
 (* 
@@ -73,40 +73,40 @@ Section Wcbv.
   Inductive eval (Γ : environment) : term -> value -> Type :=
   (** Reductions *)
   | eval_var na v :
-     lookup Γ na = Some v ->
-     eval Γ (tVar na) v
+    lookup Γ na = Some v ->
+    eval Γ (tVar na) v
 
   | eval_box a t t' :
-      eval Γ a vBox ->
-      eval Γ t t' ->
-      eval Γ (tApp a t) vBox
+    eval Γ a vBox ->
+    eval Γ t t' ->
+    eval Γ (tApp a t) vBox
 
   (** Beta *)
   | eval_beta f na b a a' res Γ' :
-      eval Γ f (vClos na b Γ') ->
-      eval Γ a a' ->
-      eval (add na a' Γ') b res ->
-      eval Γ (tApp f a) res
+    eval Γ f (vClos na b Γ') ->
+    eval Γ a a' ->
+    eval (add na a' Γ') b res ->
+    eval Γ (tApp f a) res
 
   | eval_lambda na b : 
-      eval Γ (tLambda (nNamed na) b) (vClos na b Γ)
+    eval Γ (tLambda (nNamed na) b) (vClos na b Γ)
 
   (** Let *)
   | eval_zeta na b0 b0' b1 res :
-      eval Γ b0 b0' ->
-      eval (add na b0' Γ) b1 res ->
-      eval Γ (tLetIn (nNamed na) b0 b1) res
+    eval Γ b0 b0' ->
+    eval (add na b0' Γ) b1 res ->
+    eval Γ (tLetIn (nNamed na) b0 b1) res
 
   (** Case *)
   | eval_iota_block ind pars cdecl discr c args brs br res nms :
-      eval Γ discr (vConstruct ind c args) ->
-      constructor_isprop_pars_decl Σ ind c = Some (false, pars, cdecl) ->
-      nth_error brs c = Some br ->
-      #|args| = pars + cdecl.(cstr_nargs) ->
-      #|skipn pars args| = #|br.1| ->
-      Forall2 (fun x y => x = nNamed y) br.1 nms ->
-      eval (add_multiple nms ((* List.rev  *)(skipn pars args)) Γ) br.2 res ->
-      eval Γ (tCase (ind, pars) discr brs) res
+    eval Γ discr (vConstruct ind c args) ->
+    constructor_isprop_pars_decl Σ ind c = Some (false, pars, cdecl) ->
+    nth_error brs c = Some br ->
+    #|args| = pars + cdecl.(cstr_nargs) ->
+            #|skipn pars args| = #|br.1| ->
+                                         Forall2 (fun x y => x = nNamed y) br.1 nms ->
+                                         eval (add_multiple nms ((* List.rev  *)(skipn pars args)) Γ) br.2 res ->
+                                         eval Γ (tCase (ind, pars) discr brs) res
 
   (** Fix unfolding, without guard *)
   | eval_fix_unfold f mfix idx a av fn res Γ' Γ'' na na' b :
@@ -117,22 +117,22 @@ Section Wcbv.
     eval Γ (tApp f a) res
 
   | eval_fix mfix idx nms : 
-      Forall2 (fun d n => nNamed n = d.(dname)) mfix nms ->
-      eval Γ (tFix mfix idx) (vRecClos (map2 (fun n d => (n, d.(dbody))) nms mfix) idx Γ)
+    Forall2 (fun d n => nNamed n = d.(dname)) mfix nms ->
+    eval Γ (tFix mfix idx) (vRecClos (map2 (fun n d => (n, d.(dbody))) nms mfix) idx Γ)
 
   (** Constant unfolding *)
   | eval_delta c decl body (isdecl : declared_constant Σ c decl) res :
-      decl.(cst_body) = Some body ->
-      eval Γ body res ->
-      eval Γ (tConst c) res
+    decl.(cst_body) = Some body ->
+    eval Γ body res ->
+    eval Γ (tConst c) res
 
   (** Constructor congruence: we do not allow over-applications *)
   | eval_construct_block ind c mdecl idecl cdecl args args' a a' : 
     lookup_constructor Σ ind c = Some (mdecl, idecl, cdecl) ->
     #|args| < cstr_arity mdecl cdecl ->
-    eval Γ (tConstruct ind c args) (vConstruct ind c args') ->
-    eval Γ a a' ->
-    eval Γ (tConstruct ind c (args ++ [a])) (vConstruct ind c (args' ++ [a'])).
+            eval Γ (tConstruct ind c args) (vConstruct ind c args') ->
+            eval Γ a a' ->
+            eval Γ (tConstruct ind c (args ++ [a])) (vConstruct ind c (args' ++ [a'])).
 
 End Wcbv.
 
@@ -141,7 +141,9 @@ Definition ident_of_name (na : name) : ident :=
 
 Reserved Notation "Γ ;;; E ⊩ s ~ t" (at level 50, E, s, t at next level).
 
-Inductive represents : list ident -> environment -> term -> term -> Type :=
+Unset Elimination Schemes.
+
+Inductive represents : list ident -> environment -> term -> term -> Set :=
 | represents_tBox Γ E : Γ ;;; E ⊩ tBox ~ tBox
 | represents_bound_tRel Γ n na E : nth_error Γ n = Some na -> Γ ;;; E ⊩ tVar na ~ tRel n
 | represents_unbound_tRel E na v Γ s : lookup E na = Some v -> represents_value v s -> Γ ;;; E ⊩ tVar na ~ s
@@ -149,185 +151,410 @@ Inductive represents : list ident -> environment -> term -> term -> Type :=
 | represents_tLetIn Γ E na b0 b1 na' b0' b1' : Γ ;;; E ⊩ b0 ~ b0' -> (na :: Γ) ;;; E ⊩ b1 ~ b1' -> Γ ;;; E ⊩ tLetIn (nNamed na) b0 b1 ~ tLetIn na' b0' b1'
 | represents_tApp Γ E s s' t t' : Γ ;;; E ⊩ s ~ s' -> Γ ;;; E ⊩ t ~ t' -> Γ ;;; E ⊩ tApp s t ~ tApp s' t'
 | represents_tConst Γ E c : Γ ;;; E ⊩ tConst c ~ tConst c
-| represents_tConstruct Γ E ind i args args' : All2 (represents Γ E) args args' -> Γ ;;; E ⊩ tConstruct ind i args ~ tConstruct ind i args'
-| represents_tCase Γ E ind discr discr' brs brs' allnms :
+| represents_tConstruct Γ E ind i args args' : All2_Set (represents Γ E) args args' -> Γ ;;; E ⊩ tConstruct ind i args ~ tConstruct ind i args'
+| represents_tCase Γ E ind discr discr' brs brs' :
   Γ ;;; E ⊩ discr ~ discr' ->
-  (All3 (fun b b' nms => All2 (fun n n' => n = nNamed n') b.1 nms × ((nms ++ Γ) ;;; E ⊩ (b.2) ~ (b'.2))) brs brs' allnms) ->
+  (All2_Set (fun b b' => {nms & (All2_Set (fun n n' => n = nNamed n') b.1 nms × ((nms ++ Γ) ;;; E ⊩ (b.2) ~ (b'.2)))}) brs brs') ->
   Γ ;;; E  ⊩ tCase ind discr brs ~ tCase ind discr' brs'
 | represents_tFix Γ E mfix mfix' idx nms  :
-   All2 (fun d n => d.(dname) = nNamed n) mfix nms ->
-   All2 (fun d d' => (nms ++ Γ) ;;; E ⊩ d.(dbody) ~ d'.(dbody)) mfix mfix' ->
-   Γ ;;; E ⊩ tFix mfix idx ~ tFix mfix' idx
-with represents_value : value -> term -> Type :=
+  All2_Set (fun d n => d.(dname) = nNamed n) mfix nms ->
+  All2_Set (fun d d' => (nms ++ Γ) ;;; E ⊩ d.(dbody) ~ d'.(dbody)) mfix mfix' ->
+  Γ ;;; E ⊩ tFix mfix idx ~ tFix mfix' idx
+with represents_value : value -> term -> Set :=
 | represents_value_tBox : represents_value vBox tBox
 | represents_value_tClos na E s t na' : [na] ;;; E ⊩ s ~ t -> represents_value (vClos na s E) (tLambda na' t)
-| represents_value_tConstruct vs ts ind c : All2 represents_value vs ts -> represents_value (vConstruct ind c vs) (tConstruct ind c ts)
+| represents_value_tConstruct vs ts ind c : All2_Set represents_value vs ts -> represents_value (vConstruct ind c vs) (tConstruct ind c ts)
 | represents_value_tFix vfix i E mfix :
-    All2 (fun v d => map fst vfix ;;; (add_multiple (map fst vfix) (fix_env vfix E) E) ⊩ snd v ~ d.(dbody)) vfix mfix -> represents_value (vRecClos vfix i E) (tFix mfix i)
+  All2_Set (fun v d => map fst vfix ;;; (add_multiple (map fst vfix) (fix_env vfix E) E) ⊩ snd v ~ d.(dbody)) vfix mfix -> represents_value (vRecClos vfix i E) (tFix mfix i)
 where "Γ ;;; E ⊩ s ~ t" := (represents Γ E s t).
 
-Print represents_ind.
+Program Definition represents_ind :=
+  (λ (P : ∀ (l : list ident) (e : environment) (t t0 : term),
+	       l;;; e ⊩ t ~ t0 → Type) (P0 : ∀ (v : value) (t : term),
+         represents_value v t → Type) 
+     (f : ∀ (Γ : list ident) (E : environment),
+         P Γ E tBox tBox (represents_tBox Γ E)) (f0 : 
+       ∀ (Γ : list ident) 
+         (n : nat) 
+         (na : ident) 
+         (E : environment) 
+         (e : 
+           nth_error Γ n = Some na),
+         P Γ E 
+           (tVar na) 
+           (tRel n)
+           (represents_bound_tRel Γ n
+              na E e)) 
+     (f1 : ∀ (E : environment) (na : string) (v : value) 
+             (Γ : list ident) (s : term) (e : lookup E na = Some v) 
+             (r : represents_value v s),
+         P0 v s r
+         → P Γ E (tVar na) s (represents_unbound_tRel E na v Γ s e r)) 
+     (f2 : ∀ (Γ : list ident) (E : environment) (na : ident) 
+             (na' : name) (b b' : term) (r : (na :: Γ);;; E ⊩ b ~ b'),
+         P (na :: Γ) E b b' r
+         → P Γ E (tLambda (nNamed na) b) (tLambda na' b')
+             (represents_tLambda Γ E na na' b b' r)) 
+     (f3 : ∀ (Γ : list ident) (E : environment) (na : ident) 
+             (b0 b1 : term) (na' : name) (b0' b1' : term) 
+             (r : Γ;;; E ⊩ b0 ~ b0'),
+         P Γ E b0 b0' r
+         → ∀ r0 : (na :: Γ);;; E ⊩ b1 ~ b1',
+           P (na :: Γ) E b1 b1' r0
+           → P Γ E (tLetIn (nNamed na) b0 b1) (tLetIn na' b0' b1')
+               (represents_tLetIn Γ E na b0 b1 na' b0' b1' r r0)) 
+     (f4 : ∀ (Γ : list ident) (E : environment) (s s' t t' : term) 
+             (r : Γ;;; E ⊩ s ~ s'),
+         P Γ E s s' r
+         → ∀ r0 : Γ;;; E ⊩ t ~ t',
+           P Γ E t t' r0
+           → P Γ E (tApp s t) (tApp s' t')
+               (represents_tApp Γ E s s' t t' r r0)) 
+     (f5 : ∀ (Γ : list ident) (E : environment) (c : kername),
+         P Γ E (tConst c) (tConst c) (represents_tConst Γ E c)) 
+     (f6 : ∀ (Γ : list ident) (E : environment) (ind : inductive) 
+             (i : nat) (args args' : list term) (a : All2_Set (represents Γ E) args args') (IH : All2_over a (fun t t' => P Γ E t t')),
+         P Γ E (tConstruct ind i args) (tConstruct ind i args')
+           (represents_tConstruct Γ E ind i args args' a)) 
+     (f7 : ∀ (Γ : list ident) (E : environment) (ind : inductive × nat) 
+             (discr discr' : term) (brs brs' : list (list name × term)) 
+             (r : Γ;;; E ⊩ discr ~ discr'),
+         P Γ E discr discr' r
+         → ∀ (a : All2_Set (λ b b' : list name × term, ∑ nms : list ident, All2_Set (λ (n : name) (n' : ident), n = nNamed n') b.1 nms × (nms ++ Γ);;; E ⊩ b.2 ~ b'.2) brs brs'),
+         forall IH : All2_over a (fun b b' H => P (projT1 H ++ Γ) E b.2 b'.2 (snd (projT2 H))),
+           P Γ E (tCase ind discr brs) (tCase ind discr' brs')
+             (represents_tCase Γ E ind discr discr' brs brs' r a)) 
+     (f8 : ∀ (Γ : list ident) (E : environment) (mfix mfix' : list (def term)) 
+             (idx : nat) (nms : list ident) (a : All2_Set
+                                                 (λ (d : def term) (n : ident),
+                                                   dname d = nNamed n) mfix nms) 
+             (a0 : All2_Set
+                     (λ d d' : def term, (nms ++ Γ);;; E ⊩ dbody d ~ dbody d')
+                     mfix mfix')
+             (IH : All2_over a0 (fun t t' : def term => P (nms ++ Γ) E (dbody t) (dbody t'))),
+         P Γ E (tFix mfix idx) (tFix mfix' idx)
+           (represents_tFix Γ E mfix mfix' idx nms a a0)) 
+     (f9 : P0 vBox tBox represents_value_tBox) (f10 : 
+       ∀ (na : ident) 
+         (E : environment) 
+         (s t : term) 
+         (na' : name) 
+         (r : 
+           [na];;; E ⊩ s ~ t),
+         P [na] E s t r
+         → P0 
+             (vClos na s E)
+             (tLambda na' t)
+             (represents_value_tClos na E
+                s t na' r)) 
+     (f11 : ∀ (vs : list value) (ts : list term) (ind : inductive) 
+              (c : nat) (a : All2_Set represents_value vs ts) (IH : All2_over a P0),
+         P0 (vConstruct ind c vs) (tConstruct ind c ts)
+           (represents_value_tConstruct vs ts ind c a)) 
+     (f12 : ∀ (vfix : list (ident × term)) (i : nat) 
+              (E : list (ident × value)) (mfix : list (def term)) 
+              (a : All2_Set (λ (v : ident × term) (d : def term), map fst vfix;;; add_multiple (map fst vfix) (fix_env vfix E) E ⊩ v.2 ~ dbody d) vfix mfix)
+              (IH : All2_over  a (fun v d => P (map fst vfix) (add_multiple (map fst vfix) (fix_env vfix E) E) v.2 (dbody d)  ) ),
+         P0 (vRecClos vfix i E) (tFix mfix i)
+           (represents_value_tFix vfix i E mfix a)),
+    fix F
+      (l : list ident) (e : environment) (t t0 : term) 
+      (r : l;;; e ⊩ t ~ t0) {struct r} : P l e t t0 r :=
+     match r as r0 in (l0;;; e0 ⊩ t1 ~ t2) return (P l0 e0 t1 t2 r0) with
+     | represents_tBox Γ E => f Γ E
+     | represents_bound_tRel Γ n na E e0 => f0 Γ n na E e0
+     | represents_unbound_tRel E na v Γ s e0 r0 =>
+         f1 E na v Γ s e0 r0 (F0 v s r0)
+     | represents_tLambda Γ E na na' b b' r0 =>
+         f2 Γ E na na' b b' r0 (F (na :: Γ) E b b' r0)
+     | represents_tLetIn Γ E na b0 b1 na' b0' b1' r0 r1 =>
+         f3 Γ E na b0 b1 na' b0' b1' r0 (F Γ E b0 b0' r0) r1
+           (F (na :: Γ) E b1 b1' r1)
+     | represents_tApp Γ E s s' t1 t' r0 r1 =>
+         f4 Γ E s s' t1 t' r0 (F Γ E s s' r0) r1 (F Γ E t1 t' r1)
+     | represents_tConst Γ E c => f5 Γ E c
+     | represents_tConstruct Γ E ind i args args' a =>
+         f6 Γ E ind i args args' a _
+     | represents_tCase Γ E ind discr discr' brs brs' r0 a =>
+         f7 Γ E ind discr discr' brs brs' r0 (F Γ E discr discr' r0) a _
+     | represents_tFix Γ E mfix mfix' idx nms a a0 =>
+         f8 Γ E mfix mfix' idx nms a a0 _
+     end
+   with F0 (v : value) (t : term) (r : represents_value v t) {struct r} :
+     P0 v t r :=
+          match r as r0 in (represents_value v0 t0) return (P0 v0 t0 r0) with
+          | represents_value_tBox => f9
+          | represents_value_tClos na E s t0 na' r0 =>
+              f10 na E s t0 na' r0 (F [na] E s t0 r0)
+          | represents_value_tConstruct vs ts ind c a => f11 vs ts ind c a _
+          | represents_value_tFix vfix i E mfix a => f12 vfix i E mfix a _
+          end
+            for
+            F).
+Obligation 1.
+  clear - a F. induction a; econstructor. eapply F. apply IHa.
+Defined.
+Obligation 2.
+  clear - a F. induction a; econstructor. eapply F. apply IHa.
+Defined.
+Obligation 3.
+  clear - a0 F. induction a0; econstructor. eapply F. eapply IHa0.
+Defined.
+Obligation 4.
+  clear - a F0. induction a; econstructor. eapply F0. eapply IHa.
+Defined.
+Obligation 5.
+  clear - a F. induction a; econstructor. eapply F. eapply IHa.
+Defined.
 
-Definition represents_ind' :=
-λ (P : ∀ (l : list ident) (e : environment) (t t0 : term),
-	     l;;; e ⊩ t ~ t0 → Prop) (f : ∀ (Γ : list ident) (E : environment),
-                                        P Γ E tBox tBox (represents_tBox Γ E)) 
-  (f0 : ∀ (Γ : list ident) (n : nat) (na : ident) 
-          (E : environment) (e : nth_error Γ n = Some na),
-          P Γ E (tVar na) (tRel n) (represents_bound_tRel Γ n na E e)) 
-  (f1 : ∀ (E : environment) (na : string) (v : value) 
-          (Γ : list ident) (s : term) (e : lookup E na = Some v) 
-          (r : represents_value v s),
-          P Γ E (tVar na) s (represents_unbound_tRel E na v Γ s e r)) 
-  (f2 : ∀ (Γ : list ident) (E : environment) (na : ident) 
-          (na' : name) (b b' : term) (r : (na :: Γ);;; E ⊩ b ~ b'),
-          P (na :: Γ) E b b' r
-          → P Γ E (tLambda (nNamed na) b) (tLambda na' b')
-              (represents_tLambda Γ E na na' b b' r)) 
-  (f3 : ∀ (Γ : list ident) (E : environment) (na : ident) 
-          (b0 b1 : term) (na' : name) (b0' b1' : term) 
-          (r : Γ;;; E ⊩ b0 ~ b0'),
-          P Γ E b0 b0' r
-          → ∀ r0 : (na :: Γ);;; E ⊩ b1 ~ b1',
-              P (na :: Γ) E b1 b1' r0
-              → P Γ E (tLetIn (nNamed na) b0 b1) (tLetIn na' b0' b1')
-                  (represents_tLetIn Γ E na b0 b1 na' b0' b1' r r0)) 
-  (f4 : ∀ (Γ : list ident) (E : environment) (s s' t t' : term) 
-          (r : Γ;;; E ⊩ s ~ s'),
-          P Γ E s s' r
-          → ∀ r0 : Γ;;; E ⊩ t ~ t',
-              P Γ E t t' r0
-              → P Γ E (tApp s t) (tApp s' t')
-                  (represents_tApp Γ E s s' t t' r r0)) 
-  (f5 : ∀ (Γ : list ident) (E : environment) (c : kername),
-          P Γ E (tConst c) (tConst c) (represents_tConst Γ E c)) 
-  (f6 : ∀ (Γ : list ident) (E : environment) (ind : inductive) 
-          (i : nat) (args args' : list term) (a : 
-                                              All2 
-                                                (represents Γ E) args args'),
-          P Γ E (tConstruct ind i args) (tConstruct ind i args')
-            (represents_tConstruct Γ E ind i args args' a)) 
-  (f7 : ∀ (Γ : list ident) (E : environment) (ind : inductive × nat) 
-          (discr discr' : term) (brs brs' : list (list name × term)) 
-          (allnms : list (list ident)) (r : Γ;;; E ⊩ discr ~ discr'),
-          P Γ E discr discr' r
-          → ∀ a : All3
-                    (λ (b b' : list name × term) (nms : list ident),
-                       All2 (λ (n : name) (n' : ident), n = nNamed n') b.1
-                         nms * ((nms ++ Γ);;; E ⊩ b.2 ~ b'.2)) brs brs'
-                    allnms,
-              P Γ E (tCase ind discr brs) (tCase ind discr' brs')
-                (represents_tCase Γ E ind discr discr' brs brs' allnms r a)) 
-  (f8 : ∀ (Γ : list ident) (E : environment) (mfix mfix' : list (def term)) 
-          (idx : nat) (nms : list ident) (a : All2
-                                                (λ (d : def term) (n : ident),
-                                                 dname d = nNamed n) mfix nms) 
-          (a0 : All2
-                  (λ d d' : def term, (nms ++ Γ);;; E ⊩ dbody d ~ dbody d')
-                  mfix mfix'),
-          P Γ E (tFix mfix idx) (tFix mfix' idx)
-            (represents_tFix Γ E mfix mfix' idx nms a a0)),
-  fix F
-    (l : list ident) (e : environment) (t t0 : term) 
-    (r : l;;; e ⊩ t ~ t0) {struct r} : P l e t t0 r :=
-    match r as r0 in (l0;;; e0 ⊩ t1 ~ t2) return (P l0 e0 t1 t2 r0) with
-    | represents_tBox Γ E => f Γ E
-    | represents_bound_tRel Γ n na E e0 => f0 Γ n na E e0
-    | represents_unbound_tRel E na v Γ s e0 r0 => f1 E na v Γ s e0 r0
-    | represents_tLambda Γ E na na' b b' r0 =>
-        f2 Γ E na na' b b' r0 (F (na :: Γ) E b b' r0)
-    | represents_tLetIn Γ E na b0 b1 na' b0' b1' r0 r1 =>
-        f3 Γ E na b0 b1 na' b0' b1' r0 (F Γ E b0 b0' r0) r1
-          (F (na :: Γ) E b1 b1' r1)
-    | represents_tApp Γ E s s' t1 t' r0 r1 =>
-        f4 Γ E s s' t1 t' r0 (F Γ E s s' r0) r1 (F Γ E t1 t' r1)
-    | represents_tConst Γ E c => f5 Γ E c
-    | represents_tConstruct Γ E ind i args args' a =>
-        f6 Γ E ind i args args' a
-    | represents_tCase Γ E ind discr discr' brs brs' allnms r0 a =>
-        f7 Γ E ind discr discr' brs brs' allnms r0 (F Γ E discr discr' r0) a
-    | represents_tFix Γ E mfix mfix' idx nms a a0 =>
-        f8 Γ E mfix mfix' idx nms a a0
-    end.
-     : ∀ P : ∀ (l : list ident) (e : environment) (t t0 : term),
-               l;;; e ⊩ t ~ t0 → Prop,
-         (∀ (Γ : list ident) (E : environment),
-            P Γ E tBox tBox (represents_tBox Γ E))
-         → (∀ (Γ : list ident) (n : nat) (na : ident) 
-              (E : environment) (e : nth_error Γ n = Some na),
-              P Γ E (tVar na) (tRel n) (represents_bound_tRel Γ n na E e))
-           → (∀ (E : environment) (na : string) (v : value) 
-                (Γ : list ident) (s : term) (e : lookup E na = Some v) 
-                (r : represents_value v s),
-                P Γ E (tVar na) s (represents_unbound_tRel E na v Γ s e r))
-             → (∀ (Γ : list ident) (E : environment) 
-                  (na : ident) (na' : name) (b b' : term) 
-                  (r : (na :: Γ);;; E ⊩ b ~ b'),
-                  P (na :: Γ) E b b' r
-                  → P Γ E (tLambda (nNamed na) b) 
-                      (tLambda na' b') (represents_tLambda Γ E na na' b b' r))
-               → (∀ (Γ : list ident) (E : environment) 
-                    (na : ident) (b0 b1 : term) (na' : name) 
-                    (b0' b1' : term) (r : Γ;;; E ⊩ b0 ~ b0'),
-                    P Γ E b0 b0' r
-                    → ∀ r0 : (na :: Γ);;; E ⊩ b1 ~ b1',
-                        P (na :: Γ) E b1 b1' r0
-                        → P Γ E (tLetIn (nNamed na) b0 b1)
-                            (tLetIn na' b0' b1')
-                            (represents_tLetIn Γ E na b0 b1 na' b0' b1' r r0))
-                 → (∀ (Γ : list ident) (E : environment) 
-                      (s s' t t' : term) (r : Γ;;; E ⊩ s ~ s'),
-                      P Γ E s s' r
-                      → ∀ r0 : Γ;;; E ⊩ t ~ t',
-                          P Γ E t t' r0
-                          → P Γ E (tApp s t) (tApp s' t')
-                              (represents_tApp Γ E s s' t t' r r0))
-                   → (∀ (Γ : list ident) (E : environment) (c : kername),
-                        P Γ E (tConst c) (tConst c) (represents_tConst Γ E c))
-                     → (∀ (Γ : list ident) (E : environment) 
-                          (ind : inductive) (i : nat) 
-                          (args args' : list term) 
-                          (a : All2 (represents Γ E) args args'),
-                          P Γ E (tConstruct ind i args)
-                            (tConstruct ind i args')
-                            (represents_tConstruct Γ E ind i args args' a))
-                       → (∀ (Γ : list ident) (E : environment) 
-                            (ind : inductive × nat) 
-                            (discr discr' : term) 
-                            (brs brs' : list (list name × term)) 
-                            (allnms : list (list ident)) 
-                            (r : Γ;;; E ⊩ discr ~ discr'),
-                            P Γ E discr discr' r
-                            → ∀ a : All3
-                                      (λ (b b' : list name × term) 
-                                         (nms : list ident),
-                                         All2
-                                           (λ (n : name) (n' : ident),
-                                              n = nNamed n') b.1 nms *
-                                         ((nms ++ Γ);;; E ⊩ b.2 ~ b'.2)) brs
-                                      brs' allnms,
-                                P Γ E (tCase ind discr brs)
-                                  (tCase ind discr' brs')
-                                  (represents_tCase Γ E ind discr discr' brs
-                                     brs' allnms r a))
-                         → (∀ (Γ : list ident) (E : environment) 
-                              (mfix mfix' : list (def term)) 
-                              (idx : nat) (nms : list ident) 
-                              (a : All2
-                                     (λ (d : def term) (n : ident),
-                                        dname d = nNamed n) mfix nms) 
-                              (a0 : All2
-                                      (λ d d' : def term,
-                                         (nms ++ Γ);;; E ⊩ dbody d ~ dbody d')
-                                      mfix mfix'),
-                              P Γ E (tFix mfix idx) 
-                                (tFix mfix' idx)
-                                (represents_tFix Γ E mfix mfix' idx nms a a0))
-                           → ∀ (l : list ident) (e : environment) 
-                               (t t0 : term) (r : l;;; e ⊩ t ~ t0),
-                               P l e t t0 r.
+Program Definition represents_value_ind :=
+  (λ (P : ∀ (l : list ident) (e : environment) (t t0 : term),
+	       l;;; e ⊩ t ~ t0 → Type) (P0 : ∀ (v : value) (t : term),
+         represents_value v t → Type) 
+     (f : ∀ (Γ : list ident) (E : environment),
+         P Γ E tBox tBox (represents_tBox Γ E)) (f0 : 
+       ∀ (Γ : list ident) 
+         (n : nat) 
+         (na : ident) 
+         (E : environment) 
+         (e : 
+           nth_error Γ n = Some na),
+         P Γ E 
+           (tVar na) 
+           (tRel n)
+           (represents_bound_tRel Γ n
+              na E e)) 
+     (f1 : ∀ (E : environment) (na : string) (v : value) 
+             (Γ : list ident) (s : term) (e : lookup E na = Some v) 
+             (r : represents_value v s),
+         P0 v s r
+         → P Γ E (tVar na) s (represents_unbound_tRel E na v Γ s e r)) 
+     (f2 : ∀ (Γ : list ident) (E : environment) (na : ident) 
+             (na' : name) (b b' : term) (r : (na :: Γ);;; E ⊩ b ~ b'),
+         P (na :: Γ) E b b' r
+         → P Γ E (tLambda (nNamed na) b) (tLambda na' b')
+             (represents_tLambda Γ E na na' b b' r)) 
+     (f3 : ∀ (Γ : list ident) (E : environment) (na : ident) 
+             (b0 b1 : term) (na' : name) (b0' b1' : term) 
+             (r : Γ;;; E ⊩ b0 ~ b0'),
+         P Γ E b0 b0' r
+         → ∀ r0 : (na :: Γ);;; E ⊩ b1 ~ b1',
+           P (na :: Γ) E b1 b1' r0
+           → P Γ E (tLetIn (nNamed na) b0 b1) (tLetIn na' b0' b1')
+               (represents_tLetIn Γ E na b0 b1 na' b0' b1' r r0)) 
+     (f4 : ∀ (Γ : list ident) (E : environment) (s s' t t' : term) 
+             (r : Γ;;; E ⊩ s ~ s'),
+         P Γ E s s' r
+         → ∀ r0 : Γ;;; E ⊩ t ~ t',
+           P Γ E t t' r0
+           → P Γ E (tApp s t) (tApp s' t')
+               (represents_tApp Γ E s s' t t' r r0)) 
+     (f5 : ∀ (Γ : list ident) (E : environment) (c : kername),
+         P Γ E (tConst c) (tConst c) (represents_tConst Γ E c)) 
+     (f6 : ∀ (Γ : list ident) (E : environment) (ind : inductive) 
+             (i : nat) (args args' : list term) (a : All2_Set (represents Γ E) args args') (IH : All2_over a (fun t t' => P Γ E t t')),
+         P Γ E (tConstruct ind i args) (tConstruct ind i args')
+           (represents_tConstruct Γ E ind i args args' a)) 
+     (f7 : ∀ (Γ : list ident) (E : environment) (ind : inductive × nat) 
+             (discr discr' : term) (brs brs' : list (list name × term)) 
+             (r : Γ;;; E ⊩ discr ~ discr'),
+         P Γ E discr discr' r
+         → ∀ a : All2_Set
+                   (λ b b' : list name × term,
+                       ∑ nms : list ident,
+                         All2_Set (λ (n : name) (n' : ident), n = nNamed n')
+                           b.1 nms × (nms ++ Γ);;; E ⊩ b.2 ~ b'.2) brs brs',
+            forall IH : All2_over a (fun b b' H => P (projT1 H ++ Γ) E b.2 b'.2 (snd (projT2 H))),
+           P Γ E (tCase ind discr brs) (tCase ind discr' brs')
+             (represents_tCase Γ E ind discr discr' brs brs' r a)) 
+     (f8 : ∀ (Γ : list ident) (E : environment) (mfix mfix' : list (def term)) 
+             (idx : nat) (nms : list ident) (a : All2_Set
+                                                 (λ (d : def term) (n : ident),
+                                                   dname d = nNamed n) mfix nms) 
+             (a0 : All2_Set
+                     (λ d d' : def term, (nms ++ Γ);;; E ⊩ dbody d ~ dbody d')
+                     mfix mfix')
+             (IH : All2_over a0 (fun t t' : def term => P (nms ++ Γ) E (dbody t) (dbody t'))),
+         P Γ E (tFix mfix idx) (tFix mfix' idx)
+           (represents_tFix Γ E mfix mfix' idx nms a a0)) 
+     (f9 : P0 vBox tBox represents_value_tBox) (f10 : 
+       ∀ (na : ident) 
+         (E : environment) 
+         (s t : term) 
+         (na' : name) 
+         (r : 
+           [na];;; E ⊩ s ~ t),
+         P [na] E s t r
+         → P0 
+             (vClos na s E)
+             (tLambda na' t)
+             (represents_value_tClos na E
+                s t na' r)) 
+     (f11 : ∀ (vs : list value) (ts : list term) (ind : inductive) 
+              (c : nat) (a : All2_Set represents_value vs ts) (IH : All2_over a P0),
+         P0 (vConstruct ind c vs) (tConstruct ind c ts)
+           (represents_value_tConstruct vs ts ind c a)) 
+     (f12 : ∀ (vfix : list (ident × term)) (i : nat) 
+              (E : list (ident × value)) (mfix : list (def term)) 
+              (a : All2_Set
+                     (λ (v : ident × term) (d : def term),
+                       map fst vfix;;;
+                         add_multiple (map fst vfix) (fix_env vfix E) E ⊩ v.2 ~
+                         dbody d) vfix mfix)
+              (IH : All2_over  a (fun v d => P (map fst vfix) (add_multiple (map fst vfix) (fix_env vfix E) E) v.2 (dbody d)  ) ),
+         P0 (vRecClos vfix i E) (tFix mfix i)
+           (represents_value_tFix vfix i E mfix a)),
+    fix F
+      (l : list ident) (e : environment) (t t0 : term) 
+      (r : l;;; e ⊩ t ~ t0) {struct r} : P l e t t0 r :=
+     match r as r0 in (l0;;; e0 ⊩ t1 ~ t2) return (P l0 e0 t1 t2 r0) with
+     | represents_tBox Γ E => f Γ E
+     | represents_bound_tRel Γ n na E e0 => f0 Γ n na E e0
+     | represents_unbound_tRel E na v Γ s e0 r0 =>
+         f1 E na v Γ s e0 r0 (F0 v s r0)
+     | represents_tLambda Γ E na na' b b' r0 =>
+         f2 Γ E na na' b b' r0 (F (na :: Γ) E b b' r0)
+     | represents_tLetIn Γ E na b0 b1 na' b0' b1' r0 r1 =>
+         f3 Γ E na b0 b1 na' b0' b1' r0 (F Γ E b0 b0' r0) r1
+           (F (na :: Γ) E b1 b1' r1)
+     | represents_tApp Γ E s s' t1 t' r0 r1 =>
+         f4 Γ E s s' t1 t' r0 (F Γ E s s' r0) r1 (F Γ E t1 t' r1)
+     | represents_tConst Γ E c => f5 Γ E c
+     | represents_tConstruct Γ E ind i args args' a =>
+         f6 Γ E ind i args args' a _
+     | represents_tCase Γ E ind discr discr' brs brs' r0 a =>
+         f7 Γ E ind discr discr' brs brs' r0 (F Γ E discr discr' r0) a _
+     | represents_tFix Γ E mfix mfix' idx nms a a0 =>
+         f8 Γ E mfix mfix' idx nms a a0 _
+     end
+   with F0 (v : value) (t : term) (r : represents_value v t) {struct r} :
+     P0 v t r :=
+          match r as r0 in (represents_value v0 t0) return (P0 v0 t0 r0) with
+          | represents_value_tBox => f9
+          | represents_value_tClos na E s t0 na' r0 =>
+              f10 na E s t0 na' r0 (F [na] E s t0 r0)
+          | represents_value_tConstruct vs ts ind c a => f11 vs ts ind c a _
+          | represents_value_tFix vfix i E mfix a => f12 vfix i E mfix a _
+          end
+            for
+            F0).
+Obligation 1.
+  clear - a F. induction a; econstructor. eapply F. eassumption.
+Defined.
+Obligation 2.
+  clear - a F. induction a; econstructor. eapply F. eassumption.
+Defined.
+Obligation 3.
+  clear - a0 F. induction a0; econstructor. eapply F. eassumption.
+Defined.
+Obligation 4.
+  clear - a F0. induction a; econstructor. eapply F0. eassumption.
+Defined.
+Obligation 5.
+  clear - a F. induction a; econstructor. eapply F. eassumption.
+Defined.
 
-Local Notation "v '⊩' s" := (represents_value v s) (at level 50).
+Definition rep_ind :=
+  (λ (P : ∀ (l : list ident) (e : environment) (t t0 : term),
+	       l;;; e ⊩ t ~ t0 → Type) (P0 : ∀ (v : value) (t : term),
+         represents_value v t → Type) 
+     (f : ∀ (Γ : list ident) (E : environment),
+         P Γ E tBox tBox (represents_tBox Γ E)) (f0 : 
+       ∀ (Γ : list ident) 
+         (n : nat) 
+         (na : ident) 
+         (E : environment) 
+         (e : 
+           nth_error Γ n = Some na),
+         P Γ E 
+           (tVar na) 
+           (tRel n)
+           (represents_bound_tRel Γ n
+              na E e)) 
+     (f1 : ∀ (E : environment) (na : string) (v : value) 
+             (Γ : list ident) (s : term) (e : lookup E na = Some v) 
+             (r : represents_value v s),
+         P0 v s r
+         → P Γ E (tVar na) s (represents_unbound_tRel E na v Γ s e r)) 
+     (f2 : ∀ (Γ : list ident) (E : environment) (na : ident) 
+             (na' : name) (b b' : term) (r : (na :: Γ);;; E ⊩ b ~ b'),
+         P (na :: Γ) E b b' r
+         → P Γ E (tLambda (nNamed na) b) (tLambda na' b')
+             (represents_tLambda Γ E na na' b b' r)) 
+     (f3 : ∀ (Γ : list ident) (E : environment) (na : ident) 
+             (b0 b1 : term) (na' : name) (b0' b1' : term) 
+             (r : Γ;;; E ⊩ b0 ~ b0'),
+         P Γ E b0 b0' r
+         → ∀ r0 : (na :: Γ);;; E ⊩ b1 ~ b1',
+           P (na :: Γ) E b1 b1' r0
+           → P Γ E (tLetIn (nNamed na) b0 b1) (tLetIn na' b0' b1')
+               (represents_tLetIn Γ E na b0 b1 na' b0' b1' r r0)) 
+     (f4 : ∀ (Γ : list ident) (E : environment) (s s' t t' : term) 
+             (r : Γ;;; E ⊩ s ~ s'),
+         P Γ E s s' r
+         → ∀ r0 : Γ;;; E ⊩ t ~ t',
+           P Γ E t t' r0
+           → P Γ E (tApp s t) (tApp s' t')
+               (represents_tApp Γ E s s' t t' r r0)) 
+     (f5 : ∀ (Γ : list ident) (E : environment) (c : kername),
+         P Γ E (tConst c) (tConst c) (represents_tConst Γ E c)) 
+     (f6 : ∀ (Γ : list ident) (E : environment) (ind : inductive) 
+             (i : nat) (args args' : list term) (a : All2_Set (represents Γ E) args args') (IH : All2_over a (fun t t' => P Γ E t t')),
+         P Γ E (tConstruct ind i args) (tConstruct ind i args')
+           (represents_tConstruct Γ E ind i args args' a)) 
+     (f7 : ∀ (Γ : list ident) (E : environment) (ind : inductive × nat) 
+             (discr discr' : term) (brs brs' : list (list name × term)) 
+             (r : Γ;;; E ⊩ discr ~ discr'),
+         P Γ E discr discr' r
+         → ∀ a : All2_Set
+                   (λ b b' : list name × term,
+                       ∑ nms : list ident,
+                         All2_Set (λ (n : name) (n' : ident), n = nNamed n')
+                           b.1 nms × (nms ++ Γ);;; E ⊩ b.2 ~ b'.2) brs brs',
+          forall IH : All2_over a (fun b b' H => P (projT1 H ++ Γ) E b.2 b'.2 (snd (projT2 H))),
+           P Γ E (tCase ind discr brs) (tCase ind discr' brs')
+             (represents_tCase Γ E ind discr discr' brs brs' r a)) 
+     (f8 : ∀ (Γ : list ident) (E : environment) (mfix mfix' : list (def term)) 
+             (idx : nat) (nms : list ident) (a : All2_Set
+                                                 (λ (d : def term) (n : ident),
+                                                   dname d = nNamed n) mfix nms) 
+             (a0 : All2_Set
+                     (λ d d' : def term, (nms ++ Γ);;; E ⊩ dbody d ~ dbody d')
+                     mfix mfix')
+             (IH : All2_over a0 (fun t t' : def term => P (nms ++ Γ) E (dbody t) (dbody t'))),
+         P Γ E (tFix mfix idx) (tFix mfix' idx)
+           (represents_tFix Γ E mfix mfix' idx nms a a0)) 
+     (f9 : P0 vBox tBox represents_value_tBox) (f10 : 
+       ∀ (na : ident) 
+         (E : environment) 
+         (s t : term) 
+         (na' : name) 
+         (r : 
+           [na];;; E ⊩ s ~ t),
+         P [na] E s t r
+         → P0 
+             (vClos na s E)
+             (tLambda na' t)
+             (represents_value_tClos na E
+                s t na' r)) 
+     (f11 : ∀ (vs : list value) (ts : list term) (ind : inductive) 
+              (c : nat) (a : All2_Set represents_value vs ts) (IH : All2_over a P0),
+         P0 (vConstruct ind c vs) (tConstruct ind c ts)
+           (represents_value_tConstruct vs ts ind c a)) 
+     (f12 : ∀ (vfix : list (ident × term)) (i : nat) 
+              (E : list (ident × value)) (mfix : list (def term)) 
+              (a : All2_Set
+                     (λ (v : ident × term) (d : def term),
+                       map fst vfix;;;
+                         add_multiple (map fst vfix) (fix_env vfix E) E ⊩ v.2 ~
+                         dbody d) vfix mfix)
+              (IH : All2_over  a (fun v d => P (map fst vfix) (add_multiple (map fst vfix) (fix_env vfix E) E) v.2 (dbody d)  ) ),
+         P0 (vRecClos vfix i E) (tFix mfix i)
+           (represents_value_tFix vfix i E mfix a)),
+    (represents_ind P P0 f f0 f1 f2 f3 f4 f5 f6 f7 f8 f9 f10 f11 f12,
+      represents_value_ind P P0 f f0 f1 f2 f3 f4 f5 f6 f7 f8 f9 f10 f11 f12)).
+
+Local Notation "'⊩' v ~ s" := (represents_value v s) (at level 50).
 Local Hint Constructors represents : core.
 Local Hint Constructors represents_value : core.
 
@@ -431,89 +658,94 @@ Fixpoint gen_many_fresh Γ nms :=
   match nms with
   | [] => []
   | nAnon :: nms => let na' := gen_fresh "wildcard" Γ in
-            na' :: gen_many_fresh (na' :: Γ) nms
+                    na' :: gen_many_fresh (na' :: Γ) nms
   | nNamed na :: nms => let na' := if in_dec (ReflectEq_EqDec _) na Γ then gen_fresh na Γ else na in
                         na' :: gen_many_fresh (na' :: Γ) nms
   end.
 
+Lemma gen_many_fresh_length Γ nms : #|gen_many_fresh Γ nms| = #|nms|.
+Proof.
+  induction nms as [ | [] ] in Γ |- *; cbn; congruence.
+Qed.
+
 Definition map_def_name := 
-λ (term : Set) g (f : term → term) (d : def term),
-  {| dname := g (dname d); dbody := f (dbody d); rarg := rarg d |}.
+  λ (term : Set) g (f : term → term) (d : def term),
+    {| dname := g (dname d); dbody := f (dbody d); rarg := rarg d |}.
 
 
 Section Map2.
 
-Context {A B C : Type}.
-Variable (f : A → B → C).
-Fixpoint map2 (l : list A) (l' : list B) {struct l} :
-	list C :=
-  match l with
-  | [] => []
-  | hd :: tl =>
-      match l' with
-      | [] => []
-      | hd' :: tl' => f hd hd' :: map2 tl tl'
-      end
-  end.
+  Context {A B C : Type}.
+  Variable (f : A → B → C).
+  Fixpoint map2 (l : list A) (l' : list B) {struct l} :
+	  list C :=
+    match l with
+    | [] => []
+    | hd :: tl =>
+        match l' with
+        | [] => []
+        | hd' :: tl' => f hd hd' :: map2 tl tl'
+        end
+    end.
 End Map2.
 
 Fixpoint annotate (s : list ident) (u : term) {struct u} : term :=
   match u with
   | tRel n => match nth_error s n with
-       | Some na => tVar na
-       | None => tRel n
-       end
+              | Some na => tVar na
+              | None => tRel n
+              end
   | tEvar ev args => tEvar ev (map (annotate s) args)
   | tLambda na M => let na' := match na with
                                | nNamed na => if in_dec (ReflectEq_EqDec _) na s then gen_fresh na s else na 
                                | nAnon => gen_fresh "wildcard" s
                                end in  
-                 tLambda (nNamed na') (annotate (na' :: s) M)
+                    tLambda (nNamed na') (annotate (na' :: s) M)
   | tLetIn na b b' => 
-                          let na' := match na with
-                               | nNamed na => if in_dec (ReflectEq_EqDec _) na s then gen_fresh na s else na 
-                               | nAnon => gen_fresh "wildcard" s
-                               end in
-  tLetIn (nNamed na') (annotate s b) (annotate (na' :: s) b')
+      let na' := match na with
+                 | nNamed na => if in_dec (ReflectEq_EqDec _) na s then gen_fresh na s else na 
+                 | nAnon => gen_fresh "wildcard" s
+                 end in
+      tLetIn (nNamed na') (annotate s b) (annotate (na' :: s) b')
   | tApp u0 v => tApp (annotate s u0) (annotate s v)
   | tConstruct ind i args => tConstruct ind i (map (annotate s) args)
   | tCase ind c brs =>
       let brs' :=
         map (λ br : list name × term, 
-          let nms := gen_many_fresh s br.1 in
-          (map nNamed nms, annotate (nms ++ s) br.2)) brs
-        in
+              let nms := gen_many_fresh s br.1 in
+              (map nNamed nms, annotate (nms ++ s) br.2)) brs
+      in
       tCase ind (annotate s c) brs'
   | tProj p c => tProj p (annotate s c)
   | tFix mfix idx =>
-     let nms := gen_many_fresh s (map dname mfix) in
-     let mfix' := map2 (fun d na => map_def_name _ (fun _ => nNamed na) (annotate (gen_many_fresh s (map dname mfix) ++ s)) d) mfix nms in
-    tFix mfix' idx
+      let nms := gen_many_fresh s (map dname mfix) in
+      let mfix' := map2 (fun d na => map_def_name _ (fun _ => nNamed na) (annotate (gen_many_fresh s (map dname mfix) ++ s)) d) mfix nms in
+      tFix mfix' idx
   | _ => u
   end.
 
 
 Definition extraction_term_flags := 
   {| has_tBox := true
-    ; has_tRel := true
-    ; has_tVar := false
-    ; has_tEvar := false
-    ; has_tLambda := true
-    ; has_tLetIn := true
-    ; has_tApp := true
-    ; has_tConst := true
-    ; has_tConstruct := true
-    ; has_tCase := true
-    ; has_tProj := false
-    ; has_tFix := true
-    ; has_tCoFix := false
+  ; has_tRel := true
+  ; has_tVar := false
+  ; has_tEvar := false
+  ; has_tLambda := true
+  ; has_tLetIn := true
+  ; has_tApp := true
+  ; has_tConst := true
+  ; has_tConstruct := true
+  ; has_tCase := true
+  ; has_tProj := false
+  ; has_tFix := true
+  ; has_tCoFix := false
   |}.
 
 Definition extraction_env_flags := 
   {| has_axioms := false;
-     term_switches := extraction_term_flags;
-     has_cstr_params := false ;
-     cstr_as_blocks := true |}.
+    term_switches := extraction_term_flags;
+    has_cstr_params := false ;
+    cstr_as_blocks := true |}.
 
 Local Existing Instance extraction_env_flags.
 
@@ -524,23 +756,50 @@ Proof.
   induction s in Γ, Hwf |- * using EInduction.term_forall_list_ind; cbn in *; rtoProp; eauto.
   - eapply Nat.ltb_lt in Hwf. destruct nth_error eqn:Eq; eauto.
     eapply nth_error_None in Eq. lia.
-  - admit.
-  - econstructor. eauto. admit.
-  - econstructor. 
-    2:{ induction m.
+  - econstructor. solve_all. clear - H1. induction H1; econstructor; eauto. eapply p, p.
+  - econstructor. eauto. solve_all. clear - Γ H0. induction H0; econstructor; eauto.
+    rename x into br. exists (gen_many_fresh Γ br.1). cbn. split.
+    + eapply All2_All2_Set. solve_all. now eapply All2_refl.
+    + eapply p. rewrite app_length gen_many_fresh_length. eapply p.
+  - eapply represents_tFix with (nms := gen_many_fresh Γ (map dname m)).
+    2:{ unfold wf_fix in Hwf. rtoProp. solve_all. eapply Nat.ltb_lt in H.
+        generalize (map_length dname m).
+        generalize (map dname m). intros nms Hnms. induction m in Γ, H0, n, H, nms, Hnms |- *.        
         + econstructor.
-        + admit.
+        + destruct nms; invs Hnms. invs H0.
+          destruct n0; cbn in *; econstructor.
+          * eapply H3. cbn. rewrite app_length gen_many_fresh_length H2. eapply H3.
+          * specialize IHm with (nms := nAnon :: nms). cbn in IHm.
+            todo "fix".
+          * cbn. todo "fix".
     }
-    admit.
+    todo "fix".
 Admitted.
 
 Lemma unfolds_bound : 
-  (forall Γ E s t, Γ ;;; E ⊩ s ~ t -> closedn #|Γ| t) /\
-  (forall v s, v ⊩ s -> closedn 0 s).
+  (forall Γ E s t, Γ ;;; E ⊩ s ~ t -> closedn #|Γ| t) ×
+    (forall v s, ⊩ v ~ s -> closedn 0 s).
+Proof.
+  refine (rep_ind _ _ _ _ _ _ _ _ _ _ _ _ _ _ _ _); intros; cbn; rtoProp; eauto.
+  - eapply Nat.ltb_lt, nth_error_Some. congruence.
+  - eapply closed_upwards; eauto. lia.
+  - solve_all. induction a; cbn in *; econstructor; firstorder.
+  - split. eauto. solve_all. induction a; cbn in *; econstructor; firstorder.
+    destruct r0 as (nms & Hl1 & Hl2). cbn in *.
+    todo "add branch length assumption".
+  - solve_all. eapply All2_Set_All2 in a.
+    enough (#|mfix'| = #|nms|) as ->. 
+    2:{ eapply All2_length in a. clear IH. eapply All2_Set_All2, All2_length in a0.
+        len. }
+    clear a. induction a0; cbn in *; econstructor.
+    rewrite app_length in IH. eapply IH.
+    eapply IHa0. eapply IH.
+  - solve_all. induction a; cbn in *; rtoProp; eauto. 
+    econstructor. cbn in *. eapply IH. eapply IHa. eapply IH.
 Admitted.
 
 Lemma represents_bound_head Γ E v s x :
-  v ⊩ s -> Γ ;;; add x v E ⊩ tVar x ~ s.
+  ⊩ v ~ s -> Γ ;;; add x v E ⊩ tVar x ~ s.
 Proof.
   intros H. invs H; econstructor; unfold lookup, add.
   all: try now econstructor.
@@ -548,20 +807,69 @@ Proof.
 Qed.
 
 Lemma represents_subst' Γ E s s' t v na :
-  v ⊩ t ->
+  ⊩ v ~ t ->
   (Γ ++ [na]) ;;; E ⊩ s ~ s' ->
-  Γ ;;; add na v E ⊩ s ~ csubst t #|Γ| s.
+  Γ ;;; add na v E ⊩ s ~ csubst t #|Γ| s'.
 Proof.
+  intros Hp Hs.
+  remember (Γ ++ [na]) as Γ' eqn:eq__d.
+  revert Γ Hp eq__d.
+  eapply @represents_ind with (e := E) (l := Γ') (t := s) (t0 := s') (P0 := fun _ _ _ => True).
+
+  all: intros; subst. all: cbn; eauto.
+  - destruct (Nat.compare #|Γ0| n) eqn:Eq.
+    + eapply Nat.compare_eq in Eq. subst. 
+      rewrite nth_error_app2 in e. 1: lia.
+      rewrite Nat.sub_diag in e. invs e.
+      econstructor; eauto. unfold lookup. cbn.
+      change (eqb na0 na0) with (na0 == na0); now rewrite eqb_refl.
+    + eapply Nat.compare_lt_iff in Eq.
+      pose proof (nth_error_Some (Γ0 ++ [na]) n) as [H _]. rewrite e in H.
+      rewrite app_length in H. forward H. congruence.
+      cbn in *. lia.
+    + eapply Nat.compare_gt_iff in Eq.
+      econstructor. rewrite nth_error_app1 in e; eauto.
+  - econstructor. instantiate (1 := v0).
+    + unfold lookup in *. cbn. change (eqb na0 na) with (na0 == na) in *.
+      destruct (eqb_spec na0 na); eauto.
+      subst. destruct List.find as [ [] | ] eqn:Ef; invs e.
+      eapply find_some in Ef as [H1 H2].
+      change (eqb na t0) with (na == t0) in *.
+      eapply eqb_eq in H2. subst.
+      todo "freshness".
+    + rewrite csubst_closed; eauto.
+      eapply closed_upwards. 
+      * now eapply unfolds_bound.
+      * lia.
+  - econstructor. eapply H; eauto.
+  - econstructor. eapply H; eauto. eapply H0; eauto.
+  - econstructor. induction a; cbn.
+    + econstructor.
+    + cbn in *. econstructor. eapply IH; eauto.
+      eapply IHa. eapply IH.
+  - econstructor. eapply H; eauto.
+    induction a; cbn.
+    + econstructor.
+    + cbn in *.
+      destruct r0 as (nms & H1 & H2).
+      destruct IH as [IH1 IH2].
+      econstructor. 2: eapply IHa. 2: eapply IH2.
+      exists nms. split. eauto.
+      specialize (IH1 (nms ++ Γ0)).
+      rewrite app_length in IH1.
+      assert (#|y.1| = #|x.1|) as -> by todo "add branch length in rep".
+      eapply All2_Set_All2 in H1 as HH. eapply All2_length in HH as ->.
+      eapply IH1. eauto. cbn. now rewrite <- app_assoc.
+  - econstructor; eauto. todo "fix".
 Admitted.
 
-Lemma represents_subst E s s' t v na :
-  v ⊩ t ->
-  ([na]) ;;; E ⊩ s ~ s' ->
-  [] ;;; add na v E ⊩ s ~ csubst t 0 s.
+Lemma represents_subst E s s' t v na : 
+  ⊩ v ~ t ->
+  [na] ;;; E ⊩ s ~ s' ->
+  [] ;;; add na v E ⊩ s ~ csubst t 0 s'.
 Proof.
-Admitted.
-
-Print WcbvFlags.
+  eapply represents_subst' with (Γ := []).
+Qed.
 
 Definition extraction_wcbv_flags :=
   {| with_prop_case := false ; with_guarded_fix := false ; with_constructor_as_block := true |}.
@@ -573,7 +881,7 @@ Lemma eval_represents_value Σ s t :
 Proof.
   intros Heval v Hv.
   induction Heval in v, Hv |- *; inv Hv; eauto.
-  econstructor. rename X into Hall.
+  econstructor. rename H1 into Hall.
   clear - a iha Hall.
   induction a in vs, Hall, iha |- *; cbn in *; invs Hall.
   - econstructor.
@@ -604,19 +912,19 @@ Fixpoint sunny Γ (t : term) : bool :=
   | tEvar ev args => List.forallb (sunny Γ) args
   | tLambda (nNamed na) M => fresh na Γ && sunny (na :: Γ) M
   | tApp u v => sunny Γ u && sunny Γ v
-  | tLetIn (nNamed na) b b' => fresh na Γ && sunny Γ b && sunny (na :: Γ) b'd
+  | tLetIn (nNamed na) b b' => fresh na Γ && sunny Γ b && sunny (na :: Γ) b'
   | tCase ind c brs =>
       forallb (fun br => let names := flat_map (fun x => match x with nNamed na => [na] | _ => [] end) br.1 in
-                        forallb (fun x => match x with nNamed _ => true | _ => false end) br.1 
-                      && dupfree names
-                      && sunny (names ++ Γ) br.2) brs
+                         forallb (fun x => match x with nNamed _ => true | _ => false end) br.1 
+                         && dupfree names
+                         && sunny (names ++ Γ) br.2) brs
       && sunny Γ c 
   | tProj p c => sunny Γ c
   | tFix mfix idx =>
       forallb (fun x => match x.(dname) with nNamed _ => true | _ => false end) mfix
-    && let names := flat_map (fun d => match d.(dname) with nNamed i => [i] | _ => [] end) mfix in
-    dupfree names &&
-    forallb (test_def (sunny (names ++ Γ))) mfix
+      && let names := flat_map (fun d => match d.(dname) with nNamed i => [i] | _ => [] end) mfix in
+         dupfree names &&
+           forallb (test_def (sunny (names ++ Γ))) mfix
   | tConstruct _ _ args => forallb (sunny Γ) args
   | tConst _ => true
   | _ => false
@@ -640,6 +948,19 @@ Proof.
     + eauto.
 Qed.
 
+Lemma declared_constant_All P Σ c decl : 
+  All (P ∘ snd) Σ ->
+  declared_constant Σ c decl ->
+  P (ConstantDecl decl).
+Proof.
+  induction 1; unfold declared_constant; cbn.
+  - congruence.
+  - destruct x as [kn decl']; cbn.
+    destruct (c == kn) eqn:E.
+    + inversion 1; subst. eauto.
+    + eauto.
+Qed.
+
 Local Hint Constructors All : core.
 
 Lemma eval_wf Σ E s v : 
@@ -656,7 +977,8 @@ Proof.
   - econstructor; eauto.
   - eapply IHeval2. econstructor; cbn; eauto. eauto.
   - do 2 forward IHeval1; eauto. inv IHeval1.
-    eapply IHeval2; admit.
+    eapply IHeval2. todo "pars = 0".
+    admit.
   - admit.
   - admit.
   - eapply IHeval; eauto. eapply declared_constant_Forall in isdecl.
@@ -673,1518 +995,105 @@ Admitted.
 
 Lemma implication Σ E s t u :
   Forall (fun d => match d.2 with ConstantDecl (Build_constant_body (Some d)) => sunny [] d | _ => true end) Σ ->
+  All (fun d => match d.2 with ConstantDecl (Build_constant_body (Some body)) => 
+    ∑ u E, [] ;;; E ⊩ u ~ body
+  | _ => True end) Σ ->
   All (fun x => wf (snd x)) E ->
   sunny (map fst E) u -> 
   EWcbvEval.eval Σ s t ->
-  [] ;;; E ⊩ u ~ t ->
-  ∑ v, v ⊩ t × eval Σ E u v.
+  [] ;;; E ⊩ u ~ s ->
+  ∑ v, ⊩ v ~ t × eval Σ E u v.
 Proof.
-  intros HΣ HE Hsunny Heval Hrep.
-  induction Heval in u, E, Hrep, Hsunny; cbn in *; rtoProp; eauto.
+  intros HΣ HΣind HE Hsunny Heval Hrep.
+  induction Heval in u, E, Hrep, Hsunny, HE; cbn in *; rtoProp; eauto; try congruence.
   - invs Hrep.
-    + invs X.
-    + admit.
-  - admit.
+    + invs H0.
+    + cbn in Hsunny. rtoProp. edestruct IHHeval1 as (v & Hv1 & Hv2). 3: eauto. eauto. eauto. 
+      edestruct IHHeval2 as (? & ? & ?); eauto.
+      invs Hv1. eexists; split; eauto. econstructor; eauto.      
   - invs Hrep.
-    + invs X.
-    + eapply eval_to_value in Heval1 as Hval. invs Hval.
-      * invs X; cbn in *; eauto.
-      * cbn in *. congruence.
-      * invs H; cbn in *; eauto; try congruence.
-        rtoProp. edestruct IHHeval1 as (v & Hv1 & Hv2). 2: eauto. eauto.
+    + invs H0.
+    + cbn in Hsunny. rtoProp.
+      edestruct IHHeval1 as (v1 & Hv1 & Hv2). 3: eauto. eauto. eauto.
+      invs Hv1.
+      edestruct IHHeval2 as (v2 & Hv1_ & Hv2_). 3: eauto. eauto. eauto.
+      edestruct IHHeval3 as (v3 & Hv1__ & Hv2__).
+      3: eapply represents_subst; eauto.
+      { econstructor. cbn in *. eapply eval_wf in Hv2_; eauto. eapply eval_wf in Hv2; eauto. now invs Hv2. }
+      { eapply eval_wf in Hv2; eauto. invs Hv2; eauto. }
+      eexists; split; eauto. econstructor; eauto.
+  - invs Hrep.
+    + invs H0.
+    + cbn in Hsunny. rtoProp. 
+      edestruct IHHeval1 as (v1 & Hv1 & Hv2). 3: eauto. eauto. eauto.
+      edestruct IHHeval2 as (v2 & Hv1_ & Hv2_).
+      3: eapply represents_subst; eauto.
+      { econstructor. cbn in *. eapply eval_wf in Hv2; eauto. eauto. }
+      { eapply eval_wf in Hv2; eauto. }
+      eexists; split; eauto. econstructor; eauto.
+  - invs Hrep.
+    + invs H0.
+    + cbn in Hsunny. rtoProp.
+      edestruct IHHeval1 as (v & Hv1 & Hv2). 3,1,2: eauto.
+      edestruct IHHeval2 as (v2 & Hv1_ & Hv2_).
+      3,1,2: admit. admit.
+  - todo "fix".
+  - invs Hrep. 
+    + invs H0.
+    + cbn in *. rtoProp.
+      edestruct IHHeval1 as (v1 & Hv1 & Hv2); eauto.
+      invs Hv1; destruct args using rev_ind; cbn in *; try congruence.
+      all: match goal with [H : _ = mkApps _ _ |- _ ] => now rewrite mkApps_app in H end.
+  - invs Hrep. invs H0.
+  - invs Hrep.
+    + invs H0.
+    + eapply declared_constant_Forall in isdecl as csunny.
+      2: eapply Forall_impl. 2: eauto.
+      2: { cbn. intros [] ?. cbn in *.  exact H. }
+      cbn in *. destruct decl; cbn in *.
+      eapply declared_constant_All in isdecl as cind.
+      2: eapply All_impl. 2: eauto.
+      2: { cbn. intros [] ?. cbn in *.  exact X. }
+      cbn in *. rewrite e in csunny cind.
+      subst. destruct cind as (u & e & Hu).
+     edestruct IHHeval as (v & Hv1 & Hv2); eauto.
+     cbn; eauto.
+     todo "rule for const, maybe in empty env?".      
+  - invs Hrep. invs H0.
+  - invs Hrep.
+    + invs H0. eexists. split. 2:{ econstructor. eauto. }
+      econstructor. induction a in vs, H3 |- *.
+      * invs H3. econstructor.
+      * invs H3. econstructor. todo "eval represents". eauto.
+    + assert (∑ vs, All2 (fun v t => ⊩ v ~ t) vs args' × All2 (fun v u => eval Σ E u v) vs args0) as (vs & Hvs & Hvs').
+      * cbn in Hsunny. rtoProp. induction a in iha, H3, args0, Hsunny |- *.
+        -- invs H3. exists []. split; econstructor.
+        -- invs H3. invs iha.
+           edestruct IHa as (vs & Hv1 & Hv2). 2: eauto. 2: eauto.
+           cbn in Hsunny; now rtoProp.
+           edestruct X. 3: eauto. eauto. eauto. cbn in Hsunny; now rtoProp.
+           eexists (_ :: _). split. econstructor.
+           todo "eval_represents".
+           eauto. econstructor; eauto. eapply p.
+      * eexists. split. econstructor. eapply All2_All2_Set; eauto.
+        todo "rule missing for empty block".
+  - invs Hrep.
+    + invs H0.
+    + cbn in Hsunny. rtoProp.
+      eapply eval_to_value in Heval1 as Hval. invs Hval.
+      * destruct f'; cbn in *; try congruence.           
+        edestruct IHHeval1 as (v & Hv1 & Hv2). 3: eauto. eauto. eauto. invs Hv1.
+      * invs H4; cbn in *; eauto.
+      * invs H1; cbn in *; eauto; try congruence.
+        rtoProp. edestruct IHHeval1 as (v & Hv1 & Hv2). 3: eauto. eauto. eauto.
         invs Hv1; destruct args using rev_ind; cbn in *; try congruence.
-        all: now rewrite mkApps_app in H4.
+        all: match goal with [H : _ = mkApps _ _ |- _ ] => now rewrite mkApps_app in H end.
   - invs Hrep; cbn in *; try congruence; rtoProp.
     + econstructor. split; eauto. econstructor.
     + destruct args'; congruence.
     + solve_all. eexists. split. 2: econstructor; solve_all.
-      econstructor. admit. 
+      instantiate (1 := nms).
+      econstructor. 2:{ eapply All2_Set_All2 in H. solve_all. }
+      eapply All2_Set_All2 in H, H0. eapply All2_All2_Set. solve_all.
+      clear - H H0. revert H. todo "fix".
 Admitted.
-
-
-Scheme repTerm_ind := Induction for represents Sort Type
-with repValue_ind := Induction for represents_value Sort Type.
-
-Combined Scheme rep_ind from repTerm_ind, repValue_ind.
-
-Print rep_ind.
-
-
-
-
-Forall (fun x : string * value => wf (snd x)) E ->
-sunny (map fst E) u ->
-s ⇓ t -> u,E,[] ⊢ s -> exists p, E ⊢ u ⇓ p /\ p ⊩ t.
-    
-    
-- 
-  - eautpo u eapply IHeval2; eauto using Forall.
-
-  
-
-
-  Hint Constructors eval : core.
-  Derive Signature for eval.
-  Derive NoConfusionHom for term.
-  
-  (** Characterization of values for this reduction relation.
-      Only constructors and cofixpoints can accumulate arguments.
-      All other values are atoms and cannot have arguments:
-      - box
-      - abstractions
-      - constant constructors
-      - unapplied fixpoints and cofixpoints
-   *)
-
-   Variant value_head (nargs : nat) : term -> Type :=
-   | value_head_cstr ind c mdecl idecl cdecl :
-     with_constructor_as_block = false ->
-     lookup_constructor Σ ind c = Some (mdecl, idecl, cdecl) ->
-     nargs <= cstr_arity mdecl cdecl ->
-     value_head nargs (tConstruct ind c [])
-   | value_head_cofix mfix idx : value_head nargs (tCoFix mfix idx)
-   | value_head_fix mfix idx rarg fn : 
-     cunfold_fix mfix idx = Some (rarg, fn) ->
-     (* If fixpoints are not guarded, we don't need to consider applied fixpoints 
-        as value heads*)
-     (if with_guarded_fix then nargs <= rarg else False) ->
-     value_head nargs (tFix mfix idx).
-   Derive Signature NoConfusion for value_head.
- 
-   Inductive value : term -> Type :=
-   | value_atom t : atom Σ t -> value t
-   | value_constructor ind c mdecl idecl cdecl args : 
-      with_constructor_as_block = true ->  
-      lookup_constructor Σ ind c = Some (mdecl, idecl, cdecl) ->
-      #|args| <= cstr_arity mdecl cdecl -> 
-      All value args -> value (tConstruct ind c args)
-   | value_app_nonnil f args : value_head #|args| f -> args <> [] -> All value args -> value (mkApps f args).
-   Derive Signature for value.
-
-End Wcbv.
-
-Global Hint Constructors value : value.
-
-Section Wcbv.
-  Context {wfl : WcbvFlags}.
-  Context {Σ : global_declarations}.
-  Notation eval := (eval Σ).
-  Notation value_head := (value_head Σ).
-  Notation value := (value Σ).
-
-  Lemma value_app f args : value_head #|args| f -> All value args -> value (mkApps f args).
-  Proof.
-    destruct args.
-    - intros [] hv; constructor; try easy. cbn [atom mkApps]. now rewrite e0.
-    - intros vh av. eapply value_app_nonnil => //.
-  Qed.
-
-  Lemma value_values_ind : forall P : term -> Type,
-      (forall t, atom Σ t -> P t) ->
-       (forall (ind : inductive) (c : nat) (mdecl : mutual_inductive_body) (idecl : one_inductive_body) (cdecl : constructor_body) 
-         (args : list term) (e : with_constructor_as_block = true) (e0 : lookup_constructor Σ ind c = Some (mdecl, idecl, cdecl)) 
-          (l : #|args| <= cstr_arity mdecl cdecl) (a : All value args) , All P args ->
-       P (tConstruct ind c args)) ->
-      (forall f args, value_head #|args| f -> args <> [] -> All value args -> All P args -> P (mkApps f args)) ->
-      forall t : term, value t -> P t.
-  Proof.
-    intros P X X0 X1.
-    fix value_values_ind 2. destruct 1.
-    - apply X; auto.
-    - eapply X0; auto; tea. clear -a value_values_ind. induction a; econstructor; auto.
-    - eapply X1; auto; tea.
-      clear v n. revert args a. fix aux 2. destruct 1. constructor; auto.
-      constructor. now eapply value_values_ind. now apply aux.
-  Defined.
-
-  Lemma value_head_nApp {nargs t} : value_head nargs t -> ~~ isApp t.
-  Proof. destruct 1; auto. Qed.
-  Hint Resolve value_head_nApp : core.
-
-  Lemma isStuckfix_nApp {t args} : isStuckFix t args -> ~~ isApp t.
-  Proof. destruct t; auto. Qed.
-  Hint Resolve isStuckfix_nApp : core.
-
-  Lemma atom_nApp {t} : atom Σ t -> ~~ isApp t.
-  Proof. destruct t; auto. Qed.
-  Hint Resolve atom_nApp : core.
-
-  Lemma value_mkApps_inv t l :
-    ~~ isApp t ->
-    value (mkApps t l) ->
-    ((l = []) /\ atom Σ t) 
-    + (l = [] × ∑ ind c mdecl idecl cdecl args, [ × with_constructor_as_block , lookup_constructor Σ ind c = Some (mdecl, idecl, cdecl),    t = tConstruct ind c args, #|args| <= cstr_arity mdecl cdecl & All value args])
-    + ([× l <> [], value_head #|l| t & All value l]).
-  Proof.
-    intros H H'. generalize_eq x (mkApps t l).
-    revert x H' t H. apply: value_values_ind.
-    - intros. subst.
-      now eapply atom_mkApps in H.
-    - intros * wcon lup len H IH t ht hcon.
-      destruct l using rev_ind.
-      + cbn in hcon. invs hcon. left. right. 
-        repeat eexists; eauto.
-      + rewrite mkApps_app in hcon. invs hcon.
-    - intros * vh nargs hargs ih t isapp appeq. 
-      move: (value_head_nApp vh) => Ht.
-      right. apply mkApps_eq_inj in appeq => //. intuition subst; auto => //.
-  Qed.
-  
-  Lemma value_mkApps_values t l :
-    value (mkApps t l) ->
-    ~~ isApp t ->
-    All value l.
-  Proof.
-    intros val not_app.
-    now apply value_mkApps_inv in val as [[(-> & ?) | [-> ] ] |[]].
-  Qed.
-  
-  Lemma eval_Construct_inv ind c args e  :
-     eval (tConstruct ind c args) e ->
-     ∑ args', e = tConstruct ind c args' × All2 eval args args'.
-  Proof.
-    intros H. depind H.
-    - edestruct IHeval1 as (args'' & [= ->] & H2); eauto.
-      repeat eexists; eauto. eapply All2_app; eauto.
-    - invs i. destruct args; invs H0. exists []. repeat econstructor.
-  Qed.    
-
-  Lemma eval_to_value e e' : eval e e' -> value e'.
-  Proof.
-    intros ev. induction ev; simpl; intros; eauto with value.
-
-    - change (tApp ?h ?a) with (mkApps h [a]).
-      rewrite -mkApps_app.
-      apply value_mkApps_inv in IHev1; [|easy].      
-      destruct IHev1 as [[(-> & _) | [-> ] ] |[]].
-      + apply value_app; auto. len.
-        cbn in *. econstructor; tea.
-        destruct with_guarded_fix => //. cbn; auto.
-      + apply value_app; auto. len.
-        cbn in *. econstructor; tea.
-        destruct with_guarded_fix => //. cbn; auto.
-      + depelim v. rewrite e0 in e. noconf e.
-        eapply value_app; auto. econstructor; tea.
-        destruct with_guarded_fix => //.
-        len; lia. apply All_app_inv; auto.
-          
-    - apply value_mkApps_inv in IHev1; [|easy].      
-      destruct IHev1 as [[(-> & _)|[-> ]] | []].
-      + cbn. eapply (value_app _ [a']); cbn; auto. econstructor; tea.
-      + cbn. eapply (value_app _ [a']); cbn; auto. econstructor; tea.
-      + rewrite -[tApp _ _](mkApps_app _ _ [a']).
-        eapply value_app. cbn; auto. econstructor; tea. cbn; len.
-        eapply All_app_inv; auto.
-    
-    - invs IHev1.
-      + invs H. destruct args'; invs H1. econstructor 2; eauto. len; lia. now econstructor.
-      + rewrite e0 in H3; invs H3.
-        eapply eval_Construct_inv in ev1 as (? & [= <-] & Hall).
-        econstructor 2; eauto. len. eapply All2_length in Hall. lia. 
-        eapply All_app_inv; eauto.
-      + destruct H1. destruct args0 using rev_ind. eauto. rewrite mkApps_app in H. invs H.
-    - destruct (mkApps_elim f' [a']).
-      eapply value_mkApps_inv in IHev1 => //.
-      destruct IHev1 as [?|[]]; intuition subst.
-      * rewrite H in i |- *. simpl in *.
-        apply (value_app f0 [a']). 
-        destruct f0; simpl in * |- *; try congruence.
-        + rewrite !negb_or /= in i; rtoProp; intuition auto.
-        + rewrite !negb_or /= in i; rtoProp; intuition auto.
-        + destruct with_guarded_fix.
-        now cbn in i. now cbn in i.
-        + constructor.
-        + econstructor; auto.
-      * destruct b0 as (ind & c & mdecl & idecl & cdecl & args & [H1 H2 H3 H4]).
-        rewrite -[tApp _ _](mkApps_app _ (firstn n l) [a']).
-        rewrite a0 in i |- *. simpl in *.
-        apply (value_app f0 [a']). 
-        destruct f0; simpl in * |- *; try congruence.
-        + rewrite !negb_or /= in i; rtoProp; intuition auto.
-        + destruct with_guarded_fix. now cbn in i. now cbn in i.
-      * rewrite -[tApp _ _](mkApps_app _ (firstn n l) [a']).
-        eapply value_app; eauto with pcuic. 2:eapply All_app_inv; auto.
-        len.
-        rewrite isFixApp_mkApps isConstructApp_mkApps // in i.
-        rewrite !negb_or in i. rtoProp; intuition auto.
-        destruct with_guarded_fix eqn:gfix.
-        { destruct v; cbn in * => //. constructor. }
-      { destruct v; cbn in * => //; try now constructor.
-        now rewrite gfix in y. }
-  Qed.
-
-  Lemma value_head_spec n t :
-    value_head n t -> (~~ (isLambda t || isBox t)).
-  Proof.
-    destruct 1; simpl => //.
-  Qed.
-
-  Lemma value_head_final n t :
-    value_head n t -> eval t t.
-  Proof.
-    destruct 1.
-    - constructor; try easy. now cbn [atom]; rewrite e0.
-    - now eapply eval_atom.
-    - now eapply eval_atom. 
-  Qed.
-
-  (** The codomain of evaluation is only values: *)
-  (*     It means no redex can remain at the head of an evaluated term. *)
-
-  Lemma value_head_spec' n t :
-    value_head n t -> (~~ (isLambda t || isBox t)) && atom Σ t.
-  Proof.
-    induction 1; auto. cbn [atom]; rewrite e0 //.
-  Qed.
-
-
-  Lemma closed_fix_substl_subst_eq {mfix idx d} : 
-    closed (tFix mfix idx) ->
-    nth_error mfix idx = Some d ->
-    subst0 (fix_subst mfix) (dbody d) = substl (fix_subst mfix) (dbody d).
-  Proof.  
-    move=> /= Hf; f_equal; f_equal.
-    have clfix : All (closedn 0) (fix_subst mfix).
-    { clear idx.
-      solve_all.
-      unfold fix_subst.
-      move: #|mfix| => n.
-      induction n. constructor.
-      constructor; auto.
-      simpl. solve_all. }
-    move: (fix_subst mfix) (dbody d) clfix.
-    clear; induction fix_subst => Hfix /= //.
-    now rewrite subst_empty.
-    move=> Ha; depelim Ha.
-    simpl in *.
-    intros hnth.
-    rewrite -IHfix_subst => //.
-    rewrite (subst_app_decomp [_]). simpl.
-    f_equal. rewrite lift_closed // closed_subst //.
-  Qed.
-
-  Lemma closed_unfold_fix_cunfold_eq mfix idx : 
-    closed (tFix mfix idx) ->
-    unfold_fix mfix idx = cunfold_fix mfix idx.
-  Proof.
-    unfold unfold_fix, cunfold_fix.
-    destruct (nth_error mfix idx) eqn:Heq => //.
-    intros cl; f_equal; f_equal.
-    now rewrite (closed_fix_substl_subst_eq cl).
-  Qed.
-
-  Lemma closed_cofix_substl_subst_eq {mfix idx d} : 
-    closed (tCoFix mfix idx) ->
-    nth_error mfix idx = Some d ->
-    subst0 (cofix_subst mfix) (dbody d) = substl (cofix_subst mfix) (dbody d).
-  Proof.  
-    move=> /= Hf; f_equal; f_equal.
-    have clfix : All (closedn 0) (cofix_subst mfix).
-    { clear idx.
-      solve_all.
-      unfold cofix_subst.
-      move: #|mfix| => n.
-      induction n. constructor.
-      constructor; auto.
-      simpl. solve_all. }
-    move: (cofix_subst mfix) (dbody d) clfix.
-    clear; induction cofix_subst => Hfix /= //.
-    now rewrite subst_empty.
-    move=> Ha; depelim Ha.
-    simpl in *.
-    intros hnth.
-    rewrite -IHcofix_subst => //.
-    rewrite (subst_app_decomp [_]). simpl.
-    f_equal. rewrite lift_closed // closed_subst //.
-  Qed.
-
-  Lemma closed_unfold_cofix_cunfold_eq mfix idx : 
-    closed (tCoFix mfix idx) ->
-    unfold_cofix mfix idx = cunfold_cofix mfix idx.
-  Proof.  
-    unfold unfold_cofix, cunfold_cofix.
-    destruct (nth_error mfix idx) eqn:Heq => //.
-    intros cl; f_equal; f_equal.
-    now rewrite (closed_cofix_substl_subst_eq cl).
-  Qed.
-
-  Lemma eval_mkApps_tCoFix mfix idx args v :
-    eval (mkApps (tCoFix mfix idx) args) v ->
-    exists args', v = mkApps (tCoFix mfix idx) args'.
-  Proof.
-    revert v.
-    induction args using List.rev_ind; intros v ev.
-    + exists [].
-      now depelim ev.
-    + rewrite mkApps_app in ev.
-      cbn in *.
-      depelim ev;
-        try (apply IHargs in ev1 as (? & ?); solve_discr).
-      * apply IHargs in ev1 as (argsv & ->).
-        exists (argsv ++ [a']).
-        now rewrite mkApps_app.
-      * easy.
-  Qed.
-  
-  Lemma eval_mkApps_tFix_inv mfix idx args v :
-   with_guarded_fix ->
-    eval (mkApps (tFix mfix idx) args) v ->
-    (exists args', v = mkApps (tFix mfix idx) args' /\ #|args| = #|args'|) \/
-    (exists n b, cunfold_fix mfix idx = Some (n, b) /\ n < #|args|).
-  Proof.
-    revert v.
-    induction args using List.rev_ind; intros wg v ev.
-    + left. exists [].
-      now depelim ev.
-    + rewrite mkApps_app in ev.
-      cbn in *.
-      depelim ev.
-      all: try (eapply IHargs in ev1 as [(? & ? & Heq) | (? & ? & ? & ?)]; eauto; rewrite ?Heq; try solve_discr;
-        len; rewrite ?Heq; rewrite Nat.add_comm; eauto 7).
-      * invs H. eauto 9.
-      * invs H. left. exists (x0 ++ [av]). rewrite mkApps_app. cbn. split. eauto. len. 
-      * subst. rewrite isFixApp_mkApps in i => //. rewrite v in i. cbn in i.
-        destruct isLambda; cbn in i; easy.
-      * invs i.
-  Qed.
-
-  Lemma value_app_inv L : value (mkApps tBox L) -> L = nil.
-  Proof.
-    intros. depelim X.
-    - destruct L using rev_ind.
-      reflexivity.
-      rewrite mkApps_app in i. inv i.
-    - EAstUtils.solve_discr.
-    - EAstUtils.solve_discr. depelim v.
-  Qed.
-
-  Lemma eval_to_mkApps_tBox_inv t argsv :
-    eval t (mkApps tBox argsv) ->
-    argsv = [].
-  Proof.
-    intros ev.
-    apply eval_to_value in ev.
-    now apply value_app_inv in ev.
-  Qed.
-
-  Lemma eval_stuck_Fix {f mfix idx args args'} :
-    with_guarded_fix ->
-    eval f (tFix mfix idx) ->
-    All2 eval args args' ->
-    isStuckFix (tFix mfix idx) args ->
-    eval (mkApps f args) (mkApps (tFix mfix idx) args').
-  Proof.
-    intros wgf evf hargs. revert args' hargs.
-    induction args using rev_ind; intros args' evargs.
-    - depelim evargs. cbn; auto.
-    - eapply All2_app_inv_l in evargs as [r1 [r2 [-> [evl evr]]]].
-      depelim evr. depelim evr.
-      rewrite !mkApps_app /=.
-      destruct cunfold_fix as [[rarg fn]|] eqn:eqc => //.
-      len; cbn. move/Nat.leb_le => hrarg.
-      eapply eval_fix_value. auto. 
-      eapply IHargs => //. unfold isStuckFix. rewrite eqc. apply Nat.leb_le; lia. auto. tea.
-      rewrite -(All2_length evl). lia.
-  Qed.
-
-  Lemma stuck_fix_value_inv argsv mfix idx narg fn :
-    value (mkApps (tFix mfix idx) argsv) -> 
-    cunfold_fix mfix idx = Some (narg, fn) ->
-    (All value argsv × isStuckFix (tFix mfix idx) argsv).
-  Proof.
-    remember (mkApps (tFix mfix idx) argsv) as tfix.
-    intros hv; revert Heqtfix.
-    move: tfix hv; apply: value_values_ind.
-    - intros * isatom eq; subst.
-      unfold atom in isatom. destruct argsv using rev_case => //.
-      split; auto. simpl. simpl in isatom. rewrite H //.
-      rewrite mkApps_app /= // in isatom.
-    - intros. destruct argsv using rev_case => //.
-      rewrite mkApps_app in Heqtfix => //.
-    - intros * vf hargs vargs ihargs eq. solve_discr => //. depelim vf. rewrite e.
-      intros [= <- <-]. destruct with_guarded_fix => //. split => //.
-      unfold isStuckFix. rewrite e. now apply Nat.leb_le.
-  Qed.
-    
-  Lemma stuck_fix_value_args argsv mfix idx narg fn :
-    value (mkApps (tFix mfix idx) argsv) ->
-    cunfold_fix mfix idx = Some (narg, fn) ->
-    #|argsv| <= narg.
-  Proof.
-    intros val unf.
-    eapply stuck_fix_value_inv in val; eauto.
-    destruct val.
-    simpl in i. rewrite unf in i.
-    now eapply Nat.leb_le in i.
-  Qed.
-
-  Lemma eval_mkApps_Construct ind c mdecl idecl cdecl f args args' :
-    with_constructor_as_block = false ->
-    lookup_constructor Σ ind c = Some (mdecl, idecl, cdecl) ->
-    eval f (tConstruct ind c []) ->
-    #|args| <= cstr_arity mdecl cdecl ->
-    All2 eval args args' ->
-    eval (mkApps f args) (mkApps (tConstruct ind c []) args').
-  Proof.
-    intros hblock hdecl evf hargs. revert args'.
-    induction args using rev_ind; intros args' evargs.
-    - depelim evargs. now cbn.
-    - eapply All2_app_inv_l in evargs as [r1 [r2 [-> [evl evr]]]].
-      depelim evr. depelim evr.
-      rewrite mkApps_app /=. len in hargs. cbn in hargs.
-      rewrite mkApps_app.
-      eapply eval_construct; tea.
-      eapply IHargs => //. lia.
-      rewrite -(All2_length evl). lia.
-  Qed.
-
-  Lemma eval_mkApps_Construct_block ind c mdecl idecl cdecl f args args' :
-    with_constructor_as_block ->
-    lookup_constructor Σ ind c = Some (mdecl, idecl, cdecl) ->
-    eval f (tConstruct ind c []) ->
-    #|args| <= cstr_arity mdecl cdecl ->
-    All2 eval args args' ->
-    eval (tConstruct ind c args) (tConstruct ind c args').
-  Proof.
-    intros hblock hdecl evf hargs. revert args'.
-    induction args using rev_ind; intros args' evargs.
-    - depelim evargs. econstructor. now cbn [atom]; rewrite hdecl.
-    - eapply All2_app_inv_l in evargs as [r1 [r2 [-> [evl evr]]]].
-      depelim evr. depelim evr.
-      eapply eval_construct_block; tea. 1: revert hargs; len. 
-      eapply IHargs => //. 1: revert hargs; len.
-  Qed.  
-
-  Lemma eval_mkApps_CoFix f mfix idx args args' :
-    eval f (tCoFix mfix idx) ->
-    All2 eval args args' ->
-    eval (mkApps f args) (mkApps (tCoFix mfix idx) args').
-  Proof.
-    intros evf hargs. revert args' hargs.
-    induction args using rev_ind; intros args' evargs.
-    - depelim evargs. cbn; auto.
-    - eapply All2_app_inv_l in evargs as [r1 [r2 [-> [evl evr]]]].
-      depelim evr. depelim evr.
-      rewrite !mkApps_app /=.
-      eapply eval_app_cong; tea. 
-      eapply IHargs => //.
-      rewrite isFixApp_mkApps // /= isConstructApp_mkApps // !negb_or. rtoProp; intuition auto.
-      apply nisLambda_mkApps => //.
-      destruct with_guarded_fix => //; eapply nisFix_mkApps => //.
-      apply nisBox_mkApps => //.
-  Qed.
-
-  Lemma eval_mkApps_tBox f args args' :
-    eval f tBox ->
-    All2 eval args args' ->
-    eval (mkApps f args) tBox.
-  Proof.
-    intros evf hargs. revert args' hargs.
-    induction args using rev_ind; intros args' evargs.
-    - depelim evargs. cbn; auto.
-    - eapply All2_app_inv_l in evargs as [r1 [r2 [-> [evl evr]]]].
-      depelim evr. depelim evr.
-      rewrite !mkApps_app /=.
-      eapply eval_box; tea.
-      eapply IHargs => //. eapply evl.
-  Qed.
-
-  Lemma eval_mkApps_cong f f' l l' :
-    eval f f' ->
-    value_head #|l| f' ->
-    All2 eval l l' ->
-    eval (mkApps f l) (mkApps f' l').
-  Proof.
-    revert l'. induction l using rev_ind; intros l' evf vf' evl.
-    depelim evl. eapply evf.
-    eapply All2_app_inv_l in evl as (?&?&?&?&?).
-    intuition auto. subst. depelim a0. depelim a0.
-    - destruct vf'.
-      * eapply eval_mkApps_Construct; tea. eapply All2_app; auto.
-      * eapply eval_mkApps_CoFix; auto. eapply All2_app; auto.
-      * destruct with_guarded_fix eqn:wgf => //.
-        eapply eval_stuck_Fix; tea. eapply All2_app; auto.
-        unfold isStuckFix; rewrite e0. now apply Nat.leb_le.
-  Qed.
-
-  Lemma value_final e : value e -> eval e e.
-  Proof.
-    move: e; eapply value_values_ind; simpl; intros; eauto with value.
-    - now constructor.
-    - assert (All2 eval args args).
-    { clear -X; induction X; constructor; auto. }
-      induction args using rev_ind. repeat econstructor.
-      cbn [atom]; now rewrite e0.
-      eapply All_app in a as [? HH]; eauto; invs HH.
-      eapply All_app in X as [? HH]; eauto; invs HH.
-      eapply All2_app_inv in X0 as [? HH]; eauto; invs HH.
-      econstructor; eauto. revert l. len. eapply IHargs; eauto. revert l. len.      
-    - assert (All2 eval args args).
-      { clear -X0; induction X0; constructor; auto. }
-      eapply eval_mkApps_cong => //. now eapply value_head_final. 
-  Qed.
-  
-  Set Equations With UIP.
-
-  Unset SsrRewrite.
-  Lemma eval_unique_sig {t v v'} :
-    forall (ev1 : eval t v) (ev2 : eval t v'),
-      {| pr1 := v; pr2 := ev1 |} = {| pr1 := v'; pr2 := ev2 |}.
-  Proof.
-    Local Ltac go :=
-      solve [
-          repeat
-            match goal with
-            | [H: _, H' : _ |- _] =>
-              specialize (H _ H');
-              try solve [apply (f_equal pr1) in H; cbn in *; solve_discr];
-              noconf H
-            end; easy].
-    intros ev.
-    revert v'.
-    depind ev; intros v' ev'.
-    - depelim ev'; try go.
-      specialize (IHev1 _ ev'1). noconf IHev1.
-      specialize (IHev2 _ ev'2). noconf IHev2. cbn in i. 
-      exfalso. destruct (@with_guarded_fix wfl); easy.
-    - depelim ev'; go.
-    - depelim ev'; go.
-    - depelim ev'; try go.
-      + specialize (IHev1 _ ev'1); noconf IHev1.
-        apply (f_equal pr1) in IHev1 as apps_eq. cbn in apps_eq.
-        apply mkApps_eq_inj in apps_eq as (eq1 & eq2); try easy.
-        noconf eq1. noconf eq2.
-        noconf IHev1.
-        pose proof e0. rewrite e5 in H. noconf H.
-        pose proof e as e'. rewrite e4 in e'. noconf e'.
-        assert (br0 = br) as -> by congruence.
-        rewrite -> (uip e e4), (uip e0 e5), (uip e1 e6), (uip e2 e7), (uip e3 e8).
-        specialize (IHev2 _ ev'2); noconf IHev2.
-        reflexivity.
-    - depelim ev'; try go.
-      + specialize (IHev1 _ ev'1); noconf IHev1.
-        pose proof e0. rewrite e5 in H. noconf H.
-        pose proof e as e'. rewrite e4 in e'. noconf e'.
-        assert (br0 = br) as -> by congruence.
-        rewrite -> (uip e e4), (uip e0 e5), (uip e1 e6), (uip e2 e7), (uip e3 e8).
-        specialize (IHev2 _ ev'2); noconf IHev2.
-        reflexivity.
-    - depelim ev'; try go.
-      + subst.
-        noconf e2.
-        simpl.
-        specialize (IHev1 _ ev'1); noconf IHev1. simpl.
-        pose proof (uip e e1). subst.
-        pose proof (uip i i0). subst i0.
-        now specialize (IHev2 _ ev'2); noconf IHev2.
-    - depelim ev'; try go.
-      + specialize (IHev1 _ ev'1).
-        pose proof (mkApps_eq_inj (f_equal pr1 IHev1) eq_refl eq_refl) as (? & <-).
-        noconf H.
-        noconf IHev1.
-        specialize (IHev2 _ ev'2); noconf IHev2.
-        assert (fn0 = fn) as -> by congruence.
-        assert (e0 = e) as -> by now apply uip.
-        rewrite (uip guarded guarded0).
-        now specialize (IHev3 _ ev'3); noconf IHev3.        
-      + specialize (IHev1 _ ev'1).
-        pose proof (mkApps_eq_inj (f_equal pr1 IHev1) eq_refl eq_refl) as (? & <-).
-        noconf H.
-        exfalso; rewrite e0 in e.
-        noconf e.
-        lia.
-      + specialize (IHev1 _ ev'1).
-        noconf IHev1.
-        exfalso.
-        rewrite guarded in i.
-        rewrite isFixApp_mkApps in i; try easy.
-        now rewrite Bool.orb_true_r in i.
-    - depelim ev'; try go.
-      + specialize (IHev1 _ ev'1).
-        pose proof (mkApps_eq_inj (f_equal pr1 IHev1) eq_refl eq_refl) as (? & <-).
-        noconf H.
-        exfalso; rewrite e0 in e.
-        noconf e.
-        lia.
-      + specialize (IHev1 _ ev'1).
-        pose proof (mkApps_eq_inj (f_equal pr1 IHev1) eq_refl eq_refl) as (? & <-).
-        noconf H.
-        noconf IHev1.
-        specialize (IHev2 _ ev'2); noconf IHev2.
-        assert (narg0 = narg) as -> by congruence.
-        assert (fn0 = fn) as -> by congruence.
-        assert (e0 = e) as -> by now apply uip.
-        rewrite (uip guarded guarded0).
-        now assert (l0 = l) as -> by now apply PCUICWcbvEval.le_irrel.
-      + specialize (IHev1 _ ev'1).
-        noconf IHev1.
-        exfalso.  rewrite guarded in i.
-        rewrite isFixApp_mkApps in i; try easy.
-        cbn in *.
-        now rewrite Bool.orb_true_r in i.
-    - depelim ev'; try go.
-      + move: (IHev1 _ ev'1).
-        eapply DepElim.simplification_sigma1 => heq IHev1'.
-        assert (narg0 = narg) as -> by congruence.
-        assert (fn0 = fn) as -> by congruence.
-        noconf IHev1'.
-        assert (e0 = e) as -> by now apply uip.
-        rewrite (uip unguarded unguarded0).
-        cbn in *; subst.
-        specialize (IHev2 _ ev'2). noconf IHev2.
-        now specialize (IHev3 _ ev'3); noconf IHev3.
-      + exfalso. rewrite unguarded in i.
-        specialize (IHev1 _ ev'1). depelim IHev1. easy.
-    - depelim ev'; try go.
-      move: (IHev1 _ ev'1).
-      eapply DepElim.simplification_sigma1 => heq IHev1'.
-      apply mkApps_eq_inj in heq as H'; auto.
-      destruct H' as (H' & <-). noconf H'.
-      assert (narg0 = narg) as -> by congruence.
-      assert (fn0 = fn) as -> by congruence.
-      noconf IHev1'.
-      assert (e0 = e) as -> by now apply uip.
-      cbn in *; subst.
-      now specialize (IHev2 _ ev'2); noconf IHev2.
-    - depelim ev'; try go.
-      move: (IHev1 _ ev'1).
-      eapply DepElim.simplification_sigma1 => heq IHev1'.
-      apply mkApps_eq_inj in heq as H'; auto.
-      destruct H' as (H' & <-). noconf H'.
-      assert (narg0 = narg) as -> by congruence.
-      assert (fn0 = fn) as -> by congruence.
-      noconf IHev1'.
-      assert (e0 = e) as -> by now apply uip.
-      cbn in *; subst.
-      now specialize (IHev2 _ ev'2); noconf IHev2.
-    - depelim ev'; try go.
-      unfold EGlobalEnv.declared_constant in *.
-      assert (decl0 = decl) as -> by congruence.
-      assert (body0 = body) as -> by congruence.
-      assert (e0 = e) as -> by now apply uip.
-      assert (isdecl0 = isdecl) as -> by now apply uip.
-      now specialize (IHev _ ev'); noconf IHev.
-    - depelim ev'; try go.
-      specialize (IHev1 _ ev'1).
-      pose proof (mkApps_eq_inj (f_equal pr1 IHev1) eq_refl eq_refl) as (? & <-).
-      noconf H. noconf IHev1.
-      assert (a0 = a) as -> by congruence.
-      pose proof e0 as e'. rewrite e4 in e'; noconf e'.
-      rewrite -> (uip e e3), (uip e0 e4).
-      pose proof e5 as e4'. rewrite e1 in e4'; noconf e4'.
-      rewrite -> (uip e1 e5), (uip e2 e6).
-      now specialize (IHev2 _ ev'2); noconf IHev2.
-    - depelim ev'; try go.
-      specialize (IHev1 _ ev'1); noconf IHev1.
-      assert (a0 = a) as -> by congruence.
-      pose proof e0 as e'. rewrite e4 in e'; noconf e'.
-      rewrite -> (uip e e3), (uip e0 e4).
-      pose proof e5 as e4'. rewrite e1 in e4'; noconf e4'.
-      rewrite -> (uip e1 e5), (uip e2 e6).
-      now specialize (IHev2 _ ev'2); noconf IHev2.
-    - depelim ev'; try go.
-      specialize (IHev _ ev'). noconf IHev.
-      rewrite (uip e e0).
-      now rewrite (uip i i0).
-    - depelim ev'; try now go.
-      + move: (IHev1 _ ev'1).
-        eapply DepElim.simplification_sigma1 => heq IHev1'.
-        apply mkApps_eq_inj in heq as H'; auto.
-        destruct H' as (H' & <-). noconf H'.
-        noconf IHev1'.
-        pose proof e0 as e'. rewrite e2 in e'; noconf e'.
-        specialize (IHev2 _ ev'2). noconf IHev2.
-        now rewrite -> (uip e e1), (uip e0 e2), (PCUICWcbvEval.le_irrel _ _ l l0).
-      + specialize (IHev1 _ ev'1). noconf IHev1.
-        exfalso. rewrite isConstructApp_mkApps in i.
-        cbn in i. rewrite !negb_or in i. rtoProp; intuition auto.
-    - depelim ev'; try go.
-      + eapply app_inj_tail in e3 as e4. destruct e4 as [-> ->].
-        rewrite (uip e3 eq_refl) in H. cbn in H. subst.
-        move: (IHev1 _ ev'1).
-        eapply DepElim.simplification_sigma1 => heq IHev1'.
-        noconf heq.
-        noconf IHev1'.
-        specialize (IHev2 _ ev'2). noconf IHev2.
-        pose proof e2 as E.
-        rewrite e0 in E. noconf E.
-        now rewrite -> (uip e e1), (uip e0 e2), (PCUICWcbvEval.le_irrel _ _ l l0).
-      + exfalso. invs i. destruct args; invs H0.
-    - depelim ev'; try go.
-      + exfalso. rewrite !negb_or in i. specialize (IHev1 _ ev'1); noconf IHev1.
-        cbn in i. rtoProp; intuition auto.
-      + exfalso. rewrite !negb_or in i. specialize (IHev1 _ ev'1); noconf IHev1.
-        cbn in i. rewrite guarded in i. rtoProp; intuition auto.
-        rewrite isFixApp_mkApps in H2 => //.
-      + exfalso. rewrite !negb_or in i. specialize (IHev1 _ ev'1); noconf IHev1.
-        cbn in i. rewrite guarded in i. rtoProp; intuition auto.
-        rewrite isFixApp_mkApps in H2 => //.
-      + exfalso. rewrite !negb_or in i. specialize (IHev1 _ ev'1); noconf IHev1.
-        cbn in i. rewrite unguarded in i. now cbn in i.
-      + exfalso. rewrite !negb_or in i. specialize (IHev1 _ ev'1); noconf IHev1.
-        cbn in i. rtoProp; intuition auto.
-        now rewrite isConstructApp_mkApps in H0.
-      + specialize (IHev1 _ ev'1); noconf IHev1.
-        specialize (IHev2 _ ev'2); noconf IHev2.
-        now assert (i0 = i) as -> by now apply uip.
-    - depelim ev'; try go.
-      2: now assert (i0 = i) as -> by now apply uip.
-      exfalso. invs i. destruct args; cbn in H0; invs H0.
-  Qed.
-
-  Lemma eval_unique {t v} :
-    forall (ev1 : eval t v) (ev2 : eval t v),
-      ev1 = ev2.
-  Proof.
-    intros ev ev'.
-    pose proof (eval_unique_sig ev ev').
-    now noconf H.
-  Qed.
-
-  Lemma eval_deterministic {t v v'} :
-    eval t v ->
-    eval t v' ->
-    v = v'.
-  Proof.
-    intros ev ev'.
-    pose proof (eval_unique_sig ev ev').
-    now noconf H.
-  Qed.
-    
-  Lemma eval_deterministic_all {t v v'} :
-    All2 eval t v ->
-    All2 eval t v' ->
-    v = v'.
-  Proof.
-    induction 1 in v' |- *; intros H; depelim H; auto. f_equal; eauto.
-    now eapply eval_deterministic.
-  Qed.
-
-  Lemma eval_trans' {e e' e''} :
-    eval e e' -> eval e' e'' -> e' = e''.
-  Proof.
-    intros ev ev'.
-    eapply eval_to_value in ev.
-    eapply value_final in ev.
-    eapply (eval_deterministic ev ev').
-  Qed.
-  
-  Lemma eval_trans {e e' e''} :
-    eval e e' -> eval e' e'' -> eval e e''.
-  Proof.
-    intros ev ev'.
-    enough (e' = e'') by now subst.
-    eapply eval_trans'; eauto.
-  Qed.
-
-  Set SsrRewrite.
-
-  Lemma eval_mkApps_inv f args v :
-    eval (mkApps f args) v ->
-    ∑ f', eval f f' ×  eval (mkApps f' args) v.
-  Proof.
-    revert f v; induction args using rev_ind; cbn; intros f v.
-    - intros ev. exists v. split => //. eapply eval_to_value in ev.
-      now eapply value_final.
-    - rewrite mkApps_app. intros ev.
-      depelim ev.
-      + specialize (IHargs _ _ ev1) as [f' [evf' evars]].
-        exists f'. split => //.
-        rewrite mkApps_app.
-        econstructor; tea.
-      + specialize (IHargs _ _ ev1) as [f' [evf' evars]].
-        exists f'. split => //.
-        rewrite mkApps_app.
-        eapply eval_beta; tea.
-      + specialize (IHargs _ _ ev1) as [f' [evf' ev]].
-        exists f'; split => //.
-        rewrite mkApps_app.
-        eapply eval_fix; tea.
-      + specialize (IHargs _ _ ev1) as [f' [evf' ev]].
-        exists f'; split => //.
-        rewrite mkApps_app.
-        eapply eval_fix_value; tea.
-      + specialize (IHargs _ _ ev1) as [f' [evf' ev]].
-        exists f'; split => //.
-        rewrite mkApps_app.
-        eapply eval_fix'; eauto.
-      + specialize (IHargs _ _ ev1) as [f' [evf' ev]].
-        exists f'; split => //.
-        rewrite mkApps_app.
-        eapply eval_construct; eauto.
-      + specialize (IHargs _ _ ev1) as [f'' [evf' ev]].
-        exists f''; split => //.
-        rewrite mkApps_app.
-        eapply eval_app_cong; tea.
-      + cbn in i. discriminate.
-  Qed.
-
-End Wcbv.
-
-(*
-Lemma eval_mkApps_inv' Σ f args v :
-  @eval target_wcbv_flags Σ (mkApps f args) v ->
-  ∑ f', @eval target_wcbv_flags Σ f f' × ∑ args', All2 (@eval target_wcbv_flags  Σ) args args' × @eval target_wcbv_flags Σ (mkApps f' args') v.
-Proof.
-  revert f v; induction args using rev_ind; cbn; intros f v.
-  - intros ev. exists v. split => //. eapply eval_to_value in ev.
-    exists []. split. econstructor. cbn.
-    now eapply value_final.
-  - rewrite mkApps_app. intros ev.
-    depelim ev.
-    + specialize (IHargs _ _ ev1) as [f' [evf' [args' [Hargs' evars]]]].
-      exists f'. split => //.
-      eexists. split. eapply All2_app; eauto.
-      rewrite mkApps_app.
-      econstructor; tea.
-      eapply value_final; eapply eval_to_value; eauto.
-    + specialize (IHargs _ _ ev1) as [f' [evf' [args' [Hargs' evars]]]].
-      exists f'. split => //.
-      eexists. split. eapply All2_app; eauto.
-      rewrite mkApps_app. 
-      eapply eval_beta; tea.
-      eapply value_final; eapply eval_to_value; eauto.
-    + specialize (IHargs _ _ ev1) as [f' [evf' ev]].
-      exists f'; split => //. (* 
-      rewrite mkApps_app.
-      eapply eval_fix; tea. *)
-    + specialize (IHargs _ _ ev1) as [f' [evf' ev]].
-      exists f'; split => //.
-      (* rewrite mkApps_app.
-      eapply eval_fix_value; tea. *)
-    + specialize (IHargs _ _ ev1) as [f' [evf' [args' [Hargs' evars]]]].
-      exists f'. split => //.
-      eexists. split. eapply All2_app; eauto.>
-      rewrite mkApps_app. 
-    
-    specialize (IHargs _ _ ev1) as [f' [evf' ev]].
-      exists f'; split => //.
-      rewrite mkApps_app.
-      eapply eval_fix'; eauto.
-    + specialize (IHargs _ _ ev1) as [f'' [evf' ev]].
-      exists f''; split => //.
-      rewrite mkApps_app.
-      eapply eval_app_cong; tea.
-    + cbn in i. discriminate.
-Qed.*)
-
-Arguments eval_unique_sig {_ _ _ _ _}.
-Arguments eval_deterministic {_ _ _ _ _}.
-Arguments eval_unique {_ _ _ _}.
-
-Section WcbvEnv.
-  Context {wfl : WcbvFlags} {efl : EEnvFlags}.
-
-  Lemma weakening_eval_env {Σ Σ'} : 
-    wf_glob Σ' -> extends Σ Σ' ->
-    forall v t, eval Σ v t -> eval Σ' v t.
-  Proof.
-    intros wf ex t v ev.
-    induction ev; try solve [econstructor; 
-      eauto using (extends_lookup_constructor wf ex), (extends_constructor_isprop_pars_decl wf ex), (extends_is_propositional wf ex)].
-    econstructor; eauto.
-    red in isdecl |- *. eauto using extends_lookup. constructor.
-    destruct t => //. cbn [atom] in i. destruct l => //. destruct lookup_constructor eqn:hl => //.
-    eapply (extends_lookup_constructor wf ex) in hl. now cbn [atom].
-  Qed.
-
-End WcbvEnv.
-
-Scheme eval_nondep := Minimality for eval Sort Prop.
-
-Fixpoint eval_depth {wfl : WcbvFlags} {Σ : EAst.global_declarations} {t1 t2 : EAst.term} (ev : eval Σ t1 t2) { struct ev } : nat.
-Proof.
-  rename eval_depth into aux.
-  destruct ev.
-  all:try match goal with
-  | [ H : eval _ _ _, H' : eval _ _ _, H'' : eval _ _ _ |- _ ] => 
-    apply aux in H; apply aux in H'; apply aux in H''; exact (S (Nat.max H (Nat.max H' H'')))
-  | [ H : eval _ _ _, H' : eval _ _ _ |- _ ] => 
-    apply aux in H; apply aux in H'; exact (S (Nat.max H H'))
-  | [ H : eval _ _ _ |- _ ] => apply aux in H; exact (S H)
-  end.
-  exact 1.
-Defined.
-
-Lemma isLambda_mkApps f l : ~~ isLambda f -> ~~ EAst.isLambda (mkApps f l).
-Proof.
-  induction l using rev_ind; simpl; auto => //.
-  intros isf; specialize (IHl isf).
-  now rewrite mkApps_app.
-Qed.
-
-Lemma isBox_mkApps f l : ~~ isBox f -> ~~ isBox (mkApps f l).
-Proof.
-  induction l using rev_ind; simpl; auto => //.
-  intros isf; specialize (IHl isf).
-  now rewrite mkApps_app.
-Qed.
-
-
-Lemma closedn_mkApps k f args : closedn k (mkApps f args) = closedn k f && forallb (closedn k) args.
-Proof.
-  induction args in f |- *; simpl; auto.
-  ring. rewrite IHargs /=. ring. 
-Qed.
-
-Lemma closed_fix_subst mfix : 
-  forallb (EAst.test_def (closedn (#|mfix| + 0))) mfix ->
-  forallb (closedn 0) (fix_subst mfix).
-Proof.
-  solve_all.
-  unfold fix_subst.
-  move: #|mfix| => n.
-  induction n. constructor.
-  cbn. rewrite H IHn //.
-Qed.
-
-Lemma closed_cofix_subst mfix : 
-  forallb (EAst.test_def (closedn (#|mfix| + 0))) mfix ->
-  forallb (closedn 0) (cofix_subst mfix).
-Proof.
-  solve_all.
-  unfold cofix_subst.
-  move: #|mfix| => n.
-  induction n. constructor.
-  cbn. rewrite H IHn //.
-Qed.
-
-Lemma closed_cunfold_fix mfix idx n f : 
-  closed (EAst.tFix mfix idx) ->
-  cunfold_fix mfix idx = Some (n, f) ->
-  closed f.
-Proof.
-  move=> cl.
-  rewrite /cunfold_fix.
-  destruct nth_error eqn:heq => //.
-  cbn in cl.
-  have := (nth_error_forallb heq cl) => cld. 
-  move=> [=] _ <-.
-  eapply closed_substl. now eapply closed_fix_subst.
-  rewrite fix_subst_length.
-  apply cld.
-Qed.
-
-Lemma closed_cunfold_cofix mfix idx n f : 
-  closed (EAst.tCoFix mfix idx) ->
-  cunfold_cofix mfix idx = Some (n, f) ->
-  closed f.
-Proof.
-  move=> cl.
-  rewrite /cunfold_cofix.
-  destruct nth_error eqn:heq => //.
-  cbn in cl.
-  have := (nth_error_forallb heq cl) => cld. 
-  move=> [=] _ <-.
-  eapply closed_substl. now eapply closed_cofix_subst.
-  rewrite cofix_subst_length.
-  apply cld.
-Qed.
-
-Lemma lookup_env_closed {Σ kn decl} : EGlobalEnv.closed_env Σ -> EGlobalEnv.lookup_env Σ kn = Some decl -> EGlobalEnv.closed_decl decl.
-Proof.
-  induction Σ; cbn => //.
-  move/andP => [] cla cle.
-  destruct (eqb_spec kn a.1).
-  move=> [= <-]. apply cla.
-  now eapply IHΣ.
-Qed.
-
-(** Evaluation preserves closedness: *)
-Lemma eval_closed {wfl : WcbvFlags} Σ : 
-  closed_env Σ ->
-  forall t u, closed t -> eval Σ t u -> closed u.
-Proof.
-  move=> clΣ t u Hc ev. move: Hc.
-  induction ev; simpl in *; auto;
-    (move/andP=> [/andP[Hc Hc'] Hc''] || move/andP=> [Hc Hc'] || move=>Hc); auto.
-  - eapply IHev3. rewrite ECSubst.closed_subst //. auto.
-    eapply closedn_subst; tea. cbn. rewrite andb_true_r. auto. cbn. auto.
-  - eapply IHev2.
-    rewrite ECSubst.closed_subst; auto.
-    eapply closedn_subst; tea. cbn. rewrite andb_true_r. auto.
-  - specialize (IHev1 Hc).
-    move: IHev1; rewrite closedn_mkApps => /andP[] _ clargs.
-    apply IHev2. rewrite /iota_red.
-    eapply closed_substl. now rewrite forallb_rev forallb_skipn.
-    len. rewrite e3. eapply nth_error_forallb in Hc'; tea.
-    now rewrite Nat.add_0_r in Hc'.
-  - specialize (IHev1 Hc).
-    apply IHev2. rewrite /iota_red.
-    eapply closed_substl. now rewrite forallb_rev forallb_skipn.
-    len. rewrite e3. eapply nth_error_forallb in Hc'; tea.
-    now rewrite Nat.add_0_r in Hc'.
-  - subst brs. cbn in Hc'. rewrite andb_true_r in Hc'.
-    eapply IHev2. eapply closed_substl.
-    eapply All_forallb, All_repeat => //.
-    now rewrite repeat_length.
-  - eapply IHev3.
-    apply/andP.
-    split; [|easy].
-    specialize (IHev1 Hc).
-    rewrite closedn_mkApps in IHev1.
-    move/andP: IHev1 => [clfix clargs].
-    rewrite closedn_mkApps clargs andb_true_r.
-    eapply closed_cunfold_fix; tea.
-  - apply andb_true_iff.
-    split; [|easy].
-    solve_all.
-  - eapply IHev3. rtoProp. split; eauto.
-    eapply closed_cunfold_fix; tea. eauto.
-  - eapply IHev2. rewrite closedn_mkApps.
-    rewrite closedn_mkApps in IHev1. 
-    specialize (IHev1 Hc). move/andP: IHev1 => [Hfix Hargs].
-    repeat (apply/andP; split; auto).
-    eapply closed_cunfold_cofix; tea. 
-  - specialize (IHev1 Hc). eapply IHev2. rewrite closedn_mkApps in IHev1 *.
-     move/andP: IHev1 => [Hfix Hargs].
-    rewrite closedn_mkApps Hargs.
-    rewrite andb_true_r.
-    eapply closed_cunfold_cofix; tea.
-  - apply IHev.
-    move/(lookup_env_closed clΣ): isdecl.
-    now rewrite /closed_decl e /=.
-  - have := (IHev1 Hc).
-    rewrite closedn_mkApps /= => clargs.
-    eapply IHev2; eauto.
-    eapply nth_error_forallb in clargs; tea.
-  - have := (IHev1 Hc). intros clargs.
-    eapply IHev2; eauto.
-    eapply nth_error_forallb in clargs; tea.
-  - have := (IHev1 Hc).
-    rewrite closedn_mkApps /= => clargs.
-    rewrite clargs IHev2 //.
-  - rtoProp; intuition auto. forward IHev1; solve_all;
-    eapply All_app in Hc; solve_all.
-    eapply All_app_inv; solve_all. invs b. econstructor. eauto. econstructor.
-  - rtoProp; intuition auto.
-Qed.
-
-Ltac forward_keep H :=
-  match type of H with
-  ?X -> _ =>
-    let H' := fresh in 
-    assert (H' : X) ; [|specialize (H H')]
-  end.
-
-Definition mk_env_flags has_ax has_pars tfl has_blocks :=  
-  {| has_axioms := has_ax;
-     has_cstr_params := has_pars;
-     term_switches := tfl ;
-     cstr_as_blocks := has_blocks |}.
-  
-Global Hint Rewrite andb_true_r andb_false_r : simplifications.
-Global Hint Rewrite orb_false_r orb_true_r : simplifications.
-
-Tactic Notation "sim" "in" hyp(H) :=
-  repeat (cbn in H; autorewrite with simplifications in H).
-Ltac sim := repeat (cbn ; autorewrite with simplifications).
-
-Lemma eval_wellformed {efl : EEnvFlags} {wfl : WcbvFlags} Σ : 
-  forall (has_app : has_tApp), (* necessary due to mkApps *)
-  efl.(cstr_as_blocks) = false ->
-  wf_glob Σ ->
-  forall t u, wellformed Σ 0 t -> eval Σ t u -> wellformed Σ 0 u.
-Proof.
-  move=> has_app blcks clΣ t u Hc ev. move: Hc.
-  induction ev; simpl in *; auto;
-    (move/andP=> [/andP[Hc Hc'] Hc''] || move/andP=> [Hc Hc'] || move=>Hc); auto.
-  all:intros; intuition auto; rtoProp; intuition auto; rtoProp; eauto using wellformed_csubst.
-  - eapply IHev2; eauto.
-    eapply wellformed_iota_red_brs; tea => //.
-    rewrite wellformed_mkApps // in H2. move/andP: H2 => [] //.
-  - eapply IHev2; eauto.
-    eapply wellformed_iota_red_brs; tea => //.
-    destruct cstr_as_blocks; solve_all.
-    destruct lookup_constructor_pars_args as [ [] | ]; rtoProp; repeat solve_all.   
-    destruct args; cbn in H3; eauto; econstructor.
-  - subst brs. eapply IHev2. sim in H0.
-    eapply wellformed_substl => //.
-    eapply All_forallb, All_repeat => //.
-    now rewrite repeat_length.
-  - eapply IHev3. apply/andP; split; [|easy].
-    rewrite wellformed_mkApps // in H. rewrite Hc /=.
-    move/andP: H => [clfix clargs].
-    rewrite wellformed_mkApps // clargs andb_true_r.
-    eapply wellformed_cunfold_fix; tea => //.
-  - eapply IHev3 => //. rtoProp; intuition auto.
-    eapply wellformed_cunfold_fix => //; tea. cbn. rewrite H H1 //.
-  - eapply IHev2. rewrite wellformed_mkApps //.
-    rewrite wellformed_mkApps // in H2. 
-    move/andP: H2 => [Hfix Hargs].
-    repeat (apply/andP; split; auto).
-    eapply wellformed_cunfold_cofix => //; tea. 
-  - eapply IHev2. rewrite wellformed_mkApps // in H *.
-    move/andP: H => [Hfix Hargs].
-    rewrite wellformed_mkApps // Hargs andb_true_r Hc Hc' /=.
-    eapply wellformed_cunfold_cofix; tea => //.
-  - apply IHev.
-    move/(lookup_env_wellformed clΣ): isdecl.
-    now rewrite /wf_global_decl /= e /=.
-  - move: H; rewrite wellformed_mkApps // /= => clargs.
-    eapply IHev2; eauto.
-    
-    move/andP: clargs => [/andP[] hasc wfc wfargs].
-    eapply nth_error_forallb in wfargs; tea.
-  - eapply IHev2.
-    eapply nth_error_forallb in e2; eauto.
-    destruct cstr_as_blocks; eauto.
-    destruct lookup_constructor_pars_args as [ [] | ]; rtoProp; repeat solve_all.   
-    destruct args; cbn in H0; eauto.
-  - destruct cstr_as_blocks; try congruence.
-    now destruct args; invs Hc''.
-Qed.
-
-Lemma remove_last_length {X} {l : list X} : 
-  #|remove_last l| = match l with nil => 0 | _ => #|l| - 1 end.
-Proof.
-  unfold remove_last. rewrite firstn_length.
-  destruct l; cbn; lia.
-Qed.
-
-Lemma remove_last_length' {X} {l : list X} : 
-  l <> nil -> 
-  #|remove_last l| = #|l| - 1.
-Proof.
-  intros. rewrite remove_last_length. destruct l; try congruence; lia.
-Qed.
- 
-Local Hint Rewrite @remove_last_length : len.
-
-Lemma eval_mkApps_tFix_inv_size {wfl : WcbvFlags} Σ mfix idx args v :
-  with_guarded_fix ->
-  forall Heval : eval Σ (mkApps (tFix mfix idx) args) v,
-  (∑ args', All2 (fun a a' => ∑ H : eval Σ a a', eval_depth H < eval_depth Heval) args args' ×
-     v = mkApps (tFix mfix idx) (args')) +
-  (∑ n b, args <> nil /\ cunfold_fix mfix idx = Some (n, b) /\ n < #|args|).
-Proof.
- revert v.
- induction args using rev_ind; intros v wg ev.
- + left. exists []. split. repeat econstructor. now depelim ev.
- + rewrite mkApps_app in ev |- *.
-   cbn in *.
-   depelim ev.
-  
-   all: try(specialize (IHargs) with (Heval := ev1); 
-    destruct IHargs as [(args' & ? & Heq) | (? & ? & ? & ? & ?)];eauto; 
-      rewrite ?Heq; try solve_discr; try congruence; try noconf H;
-     len; rewrite ?Heq; rewrite Nat.add_comm; eauto 9).
-   * right. repeat eexists. destruct args; cbn; congruence. eauto.
-     rewrite (All2_length a); lia.
-   * left. eexists. split. sq. eapply All2_app. solve_all. destruct H. unshelve eexists. eauto. cbn. lia.
-     econstructor. 2: econstructor.
-     unshelve eexists. eauto. lia.
-     now rewrite !mkApps_app.
-   * subst f'. rewrite wg in i.
-     rewrite isFixApp_mkApps /= /isFixApp /= in i.
-     rewrite !negb_or in i; rtoProp; intuition auto. now cbn in H2.
-   * now cbn in i.
-Qed.
-
-Lemma size_final {wfl : WcbvFlags} Σ t v :
-  forall He : eval Σ t v, ∑ He' : eval Σ v v, eval_depth He' <= eval_depth He.
-Proof.
-  intros He. induction He.
-  all: try now unshelve eexists; eauto; [ eapply IHHe | cbn; destruct IHHe; lia ].
-  all: try now unshelve eexists; eauto; [ eapply IHHe2 | cbn; destruct IHHe2; lia ].
-  all: try now unshelve eexists; eauto; [ eapply IHHe3 | cbn; destruct IHHe3; lia ].
-  all: try now unshelve eexists; eauto; cbn; lia.
-  - unshelve eexists. repeat econstructor. cbn; lia.
-  - unshelve eexists; eauto. eapply eval_fix_value; eauto. eapply IHHe1. eapply IHHe2. cbn. destruct IHHe1, IHHe2. lia.
-  - unshelve eexists. eapply eval_construct; eauto.
-    eapply IHHe1. eapply IHHe2. cbn. destruct IHHe1, IHHe2. cbn. lia.
-  - unshelve eexists. eapply eval_construct_block; eauto.
-   { clear - l He1. eapply eval_Construct_inv in He1 as (? & ? & ?). eapply All2_length in a. invs e. lia. } 
-     eapply IHHe1. eapply IHHe2. cbn. destruct IHHe1, IHHe2; lia.
-  - unshelve eexists. eapply eval_app_cong; eauto. eapply IHHe1. eapply IHHe2. cbn. destruct IHHe1, IHHe2. lia.
-Qed.
-
-Lemma eval_mkApps_tFix_inv_size_unguarded {wfl : WcbvFlags} Σ mfix idx args v :
-  with_guarded_fix = false ->
-  forall Heval : eval Σ (mkApps (tFix mfix idx) args) v,
-  (args = [] /\ v = tFix mfix idx)
-  + ∑ a av args' argsv, 
-    (args = a :: args')%list ×
-    All2 (fun a a' => (a = a') + (∑ H : eval Σ a a', eval_depth H < eval_depth Heval)) args' argsv ×
-    ∑ n fn, cunfold_fix mfix idx = Some (n, fn) ×
-    ∑ H : eval Σ a av, eval_depth H <= eval_depth Heval ×
-    ∑ H : eval Σ (mkApps (tApp fn av) argsv) v, eval_depth H <= eval_depth Heval.
-Proof.
- revert v.
- induction args using rev_ind; intros v wg ev.
- + left. now depelim ev.
- + rewrite mkApps_app in ev |- *.
-   cbn in *.
-   depelim ev; right.
-  
-   all: try(specialize (IHargs) with (Heval := ev1); destruct IHargs as [[-> Heq] | (a & aval & args' & argsv_ & Heqargs & Hall & n & fn_ & Hunf & Heva & Hevasz & Hev' & Hevsz')];eauto; try rewrite ?Heq; try solve_discr; try congruence;
-     len; try rewrite ?Heq; rewrite ?Nat.add_comm; eauto 9).
-   * subst. cbn. exists a, aval, (args' ++ [x])%list,(argsv_ ++ [t'])%list. split. reflexivity.
-      repeat unshelve eexists; eauto. 3:{ rewrite mkApps_app. econstructor. eauto. eapply size_final. eauto. }
-      eapply All2_app.
-      solve_all. right. destruct b. unshelve eexists; eauto. lia.
-      unshelve econstructor. right. unshelve eexists. eauto. lia. repeat econstructor.
-      cbn in *; lia.
-      cbn. generalize (mkApps_app (tApp fn_ aval) argsv_ [t']). generalize (EAst.mkApps (tApp fn_ aval) (argsv_ ++ [t'])).
-      cbn. intros. subst. cbn. destruct size_final. cbn in *. lia.
-   * subst. cbn. exists a, aval, (args' ++ [x])%list,(argsv_ ++ [a'])%list. split. reflexivity.
-     repeat unshelve eexists; eauto.
-     eapply All2_app.
-     solve_all. right. destruct b0. unshelve eexists; eauto. lia.
-   unshelve econstructor. right. unshelve eexists. eauto. lia. repeat econstructor.
-   cbn in *; lia.
-   rewrite mkApps_app. cbn. econstructor; eauto. eapply size_final; eauto.
-   cbn. generalize (mkApps_app (tApp fn_ aval) argsv_ [a']). generalize (EAst.mkApps (tApp fn_ aval) (argsv_ ++ [a'])).
-   intros. subst. cbn.
-   destruct size_final. cbn in *. lia.
-  
-   * invs Heq. exists x, av, [], []. repeat split. econstructor. repeat unshelve eexists; eauto.
-     all:cbn; lia.
-   * subst. cbn. eexists _, _, _, (argsv_ ++ [_])%list. repeat eexists. 2: eauto.
-    eapply All2_app.
-     solve_all. right. destruct b. exists x1. cbn. lia. econstructor. now left. econstructor.
-     Unshelve. 5:{ rewrite mkApps_app. eapply eval_fix'; eauto. }
-     3:tea. cbn in *; lia.
-     cbn. generalize (mkApps_app (tApp fn_ aval) argsv_ [x]). generalize (EAst.mkApps (tApp fn_ aval) (argsv_ ++ [x])). intros. subst. cbn.
-     cbn in *. lia.
-   * subst. exists a, aval, (args' ++ [x]), (argsv_ ++ [a']).
-     split => //. split.
-     { eapply All2_app.
-      - eapply All2_impl; tea; cbv beta.
-        intros ?? [eq|[H IH]]; intuition auto. right; exists H. cbn. clear -IH. cbn in *. lia.
-      - constructor; auto.
-        right; exists ev2. cbn; lia. }
-    exists n, fn_. split => //.
-    exists Heva; cbn. split => //. cbn in *; lia.
-    rewrite mkApps_app /=.
-    unshelve eexists. eapply eval_construct; tea.
-    exact (size_final _ _ _ ev2).π1.
-    cbn. destruct size_final; cbn. cbn in *. lia.
-   * subst. cbn in i. exfalso. destruct with_guarded_fix; easy.
-   * subst.  cbn. eexists _, _, _, (argsv_ ++ [_])%list. repeat eexists. 2: eauto.
-     eapply All2_app.
-     solve_all. right. destruct b. exists x1. cbn. lia. econstructor. now left. econstructor.
-     Unshelve. 4:tea. 3:{ rewrite mkApps_app. eapply eval_app_cong; eauto. }
-     cbn in *; lia.
-     cbn. generalize (mkApps_app (tApp fn_ aval) argsv_ [x]). generalize (EAst.mkApps (tApp fn_ aval) (argsv_ ++ [x])). intros. subst. cbn.
-     cbn in *. lia.
-   * subst. cbn. invs i.
-Qed.
-
-Lemma eval_mkApps_inv' {wfl : WcbvFlags} Σ f args v :
-  eval Σ (mkApps f args) v ->
-  ∑ f' args', eval Σ f f' × All2 (eval Σ) args args' × eval Σ (mkApps f' args') v.
-Proof.
-  revert f v; induction args using rev_ind; cbn; intros f v.
-  - intros ev. exists v, []. split => //. eapply eval_to_value in ev.
-    split => //. now eapply value_final.
-  - rewrite mkApps_app. intros ev.
-    depelim ev.
-    + specialize (IHargs _ _ ev1) as [f' [args' [evf' [evars res]]]].
-      exists f', (args' ++ [t']). split => //.
-      rewrite mkApps_app.
-      econstructor; tea. eapply All2_app; auto.
-      econstructor; tea. eapply value_final. now eapply eval_to_value in ev2.
-    + specialize (IHargs _ _ ev1) as [f' [args' [evf' [evars res]]]].
-      exists f', (args' ++ [a']). split => //. split; auto.
-      eapply All2_app; auto.
-      rewrite mkApps_app.
-      eapply eval_beta; tea. eapply value_final, eval_to_value; tea.
-    + specialize (IHargs _ _ ev1) as [f' [args' [evf' [evars res]]]].
-      exists f', (args' ++ [av]); split => //. split => //.
-      eapply All2_app; auto.
-      rewrite mkApps_app.
-      eapply eval_fix; tea. eapply value_final, eval_to_value; tea.
-    + specialize (IHargs _ _ ev1) as [f' [args' [evf' [evars res]]]].
-      exists f', (args' ++ [av]); split => //. split => //.
-      eapply All2_app; auto.
-      rewrite mkApps_app.
-      eapply eval_fix_value; tea. eapply value_final, eval_to_value; tea.
-    + destruct (IHargs _ _ ev1) as [f' [args' [evf' [evars res]]]].
-      exists f', (args' ++ [av]); split => //. split => //.
-      eapply All2_app; auto.
-      rewrite mkApps_app. 
-      eapply eval_fix'; eauto. eapply value_final, eval_to_value; tea.
-    + specialize (IHargs _ _ ev1) as [f'' [args' [evf' [evars res]]]].
-      exists f'', (args' ++ [a']); split => //. split => //.
-      eapply All2_app; auto.
-      rewrite mkApps_app.
-      eapply eval_construct; tea. eapply value_final, eval_to_value; tea.
-    + specialize (IHargs _ _ ev1) as [f'' [args' [evf' [evars res]]]].
-      exists f'', (args' ++ [a']); split => //. split => //.
-      eapply All2_app; auto.
-      rewrite mkApps_app.
-      eapply eval_app_cong; tea. eapply value_final, eval_to_value; tea.
-    + cbn in i. discriminate.
-Qed.
-
-Lemma eval_mkApps_Construct_inv {fl : WcbvFlags} Σ kn c args e : 
-  with_constructor_as_block = false -> 
-  eval Σ (mkApps (tConstruct kn c []) args) e -> 
-  ∑ args', [× isSome (lookup_constructor Σ kn c), (e = mkApps (tConstruct kn c []) args') & All2 (eval Σ) args args'].
-Proof.
-  intros hblock.
-  revert e; induction args using rev_ind; intros e.
-  - intros ev. depelim ev. congruence. exists []=> //.
-  - intros ev. rewrite mkApps_app /= in ev.
-    depelim ev; try solve_discr.
-    destruct (IHargs _ ev1) as [? []]. solve_discr.
-    all:try specialize (IHargs _ ev1) as [? []]; try solve_discr; try noconf H.
-    * exists (x0 ++ [a']). split => //.
-      rewrite mkApps_app /= //. eapply All2_app; eauto.
-    * subst f'. 
-      exists (x0 ++ [a'])%list.
-      rewrite mkApps_app /= //.
-      cbn in i. split => //. eapply All2_app; eauto.
-    * now cbn in i.
-Qed.
-
-Lemma eval_mkApps_Construct_block_inv {fl : WcbvFlags} Σ kn c args oargs e : 
-  with_constructor_as_block -> 
-  eval Σ (mkApps (tConstruct kn c args) oargs) e -> 
-  ∑ args', oargs = [] × (e = tConstruct kn c args') × All2 (eval Σ) args args'.
-Proof.
-  intros hblock.
-  revert e; induction oargs using rev_ind; intros e.
-  - intros ev. depelim ev. 
-    + eexists. split. reflexivity. split. reflexivity.
-      eapply eval_Construct_inv in ev1 as (? & [= <-] & ?).
-      eapply All2_app; eauto.
-    + invs i. destruct args; invs H0. exists []. repeat econstructor.
-  - intros ev. rewrite mkApps_app /= in ev.
-    depelim ev; try solve_discr.
-    all: try specialize (IHoargs _ ev1) as (? & ? & E & ?); try congruence; try solve_discr; try noconf E.
-    * subst. cbn in i. destruct with_guarded_fix; cbn in *; eauto.
-    * invs i.
-Qed. 
-
-Lemma eval_mkApps_inv_size {wfl : WcbvFlags} {Σ f args v} :
-  forall ev : eval Σ (mkApps f args) v,
-  ∑ f' args' (evf : eval Σ f f'),
-    [× eval_depth evf <= eval_depth ev,
-      All2 (fun a a' => ∑ eva : eval Σ a a', eval_depth eva < eval_depth ev) args args' &
-      ∑ evres : eval Σ (mkApps f' args') v, eval_depth evres <= eval_depth ev].
-Proof.
-  revert f v; induction args using rev_ind; cbn; intros f v.
-  - intros ev. exists v, []. exists ev => //. split => //.
-    exact (size_final _ _ _ ev).
-  - rewrite mkApps_app. intros ev.
-    depelim ev.
-    + specialize (IHargs _ _ ev1) as [f' [args' [evf' [evfs evars [evres res]]]]].
-      exists f', (args' ++ [t']). exists evf'.
-      rewrite mkApps_app. 
-      split => //. cbn. lia.
-      { eapply All2_app; auto.
-        { cbn. solve_all. destruct H as [eva evas]; exists eva. lia. }
-        constructor; auto. exists ev2. cbn; lia. }
-      unshelve econstructor; tea.
-      econstructor; tea.
-      exact (size_final _ _ _ ev2).π1. cbn.
-      destruct size_final; cbn. lia.
-    + specialize (IHargs _ _ ev1) as [f' [args' [evf' [evfs evars [evres res]]]]].
-      exists f', (args' ++ [a']). exists evf'. split => //. 
-      cbn; lia.
-      { eapply All2_app; auto.
-        { cbn. solve_all. destruct H as [eva evas]; exists eva. lia. }
-        constructor; auto. exists ev2. cbn; lia. }
-      rewrite mkApps_app.
-      unshelve eexists.
-      eapply eval_beta; tea. 
-      exact (size_final _ _ _ ev2).π1. cbn.
-      destruct size_final; cbn; lia.
-    + specialize (IHargs _ _ ev1) as [f' [args' [evf' [evfs evars [evres res]]]]].
-      exists f', (args' ++ [av]); exists evf'; split => //. 
-      cbn; lia. 
-      { eapply All2_app; auto.
-        { cbn. solve_all. destruct H as [eva evas]; exists eva. lia. }
-        constructor; auto. exists ev2. cbn; lia. }
-      rewrite mkApps_app.
-      unshelve eexists. eapply eval_fix; tea.
-      exact (size_final _ _ _ ev2).π1. cbn.
-      destruct size_final; cbn; lia.
-    + specialize (IHargs _ _ ev1) as [f' [args' [evf' [evfs evars [evres res]]]]].
-      exists f', (args' ++ [av]); exists evf'; split => //.
-      cbn; lia. 
-      { eapply All2_app; auto.
-        { cbn. solve_all. destruct H as [eva evas]; exists eva. lia. }
-        constructor; auto. exists ev2. cbn; lia. }
-      rewrite mkApps_app.
-      unshelve eexists. eapply eval_fix_value; tea.
-      exact (size_final _ _ _ ev2).π1. cbn.
-      destruct size_final; cbn; lia.
-    + destruct (IHargs _ _ ev1) as [f' [args' [evf' [evfs evars [evres res]]]]].
-      exists f', (args' ++ [av]); exists evf'; split => //.
-      cbn; lia. 
-      { eapply All2_app; auto.
-        { cbn. solve_all. destruct H as [eva evas]; exists eva. lia. }
-        constructor; auto. exists ev2. cbn; lia. }
-      rewrite mkApps_app.
-      unshelve eexists. eapply eval_fix'; tea.
-      exact (size_final _ _ _ ev2).π1. cbn.
-      destruct size_final; cbn; lia.
-    + specialize (IHargs _ _ ev1) as [f'' [args' [evf' [evfs evars [evres res]]]]].
-      exists f'', (args' ++ [a']); exists evf'; split => //.
-      cbn; lia.
-      { eapply All2_app; auto.
-        { cbn. solve_all. destruct H as [eva evas]; exists eva. lia. }
-        constructor; auto. exists ev2. cbn; lia. }
-      rewrite mkApps_app.
-      unshelve eexists. eapply eval_construct; tea.
-      exact (size_final _ _ _ ev2).π1. cbn.
-      destruct size_final; cbn; lia. 
-    + specialize (IHargs _ _ ev1) as [f'' [args' [evf' [evfs evars [evres res]]]]].
-      exists f'', (args' ++ [a']); exists evf'; split => //.
-      cbn; lia.
-      { eapply All2_app; auto.
-        { cbn. solve_all. destruct H as [eva evas]; exists eva. lia. }
-        constructor; auto. exists ev2. cbn; lia. }
-      rewrite mkApps_app.
-      unshelve eexists. eapply eval_app_cong; tea.
-      exact (size_final _ _ _ ev2).π1. cbn.
-      destruct size_final; cbn; lia. 
-    + cbn in i. discriminate.
-Qed.
-
-Lemma eval_mkApps_Construct_size {wfl : WcbvFlags} {Σ ind c args v} :
-  with_constructor_as_block = false ->
-  forall ev : eval Σ (mkApps (tConstruct ind c []) args) v,
-  ∑ args' (evf : eval Σ (tConstruct ind c []) (tConstruct ind c [])),
-    [× eval_depth evf <= eval_depth ev,
-      All2 (fun a a' => ∑ eva : eval Σ a a', eval_depth eva < eval_depth ev) args args' &
-      v = mkApps (tConstruct ind c []) args'].
-Proof.
-  intros hblock ev.
-  destruct (eval_mkApps_inv_size ev) as [f'' [args' [? []]]].
-  exists args'.
-  destruct (eval_mkApps_Construct_inv _ _ _ _ _ hblock ev) as [? []]. subst v.
-  exists (eval_atom _ (tConstruct ind c []) i).
-  cbn. split => //. destruct ev; cbn => //; auto with arith.
-  clear l.
-  eapply (eval_mkApps_Construct_inv _ _ _ [] _ hblock) in x as [? []]; auto. subst f''. depelim a1.
-  f_equal.
-  eapply eval_deterministic_all; tea.
-  eapply All2_impl; tea; cbn; eauto. now intros x y []. 
-Qed.
-
-Lemma eval_construct_size  {fl : WcbvFlags} [Σ kn c args e] : 
-  with_constructor_as_block = false ->
-  forall (ev : eval Σ (mkApps (tConstruct kn c []) args) e),
-  ∑ args', (e = mkApps (tConstruct kn c []) args') ×
-  All2 (fun x y => ∑ ev' : eval Σ x y, eval_depth ev' < eval_depth ev) args args'.
-Proof.
-  intros hblock ev; destruct (eval_mkApps_Construct_size hblock ev) as [args'[evf [_ hargs hv]]].
-  exists args'; intuition auto.
-Qed.
-
-Lemma eval_box_apps {wfl : WcbvFlags}:
-  forall (Σ' : global_declarations) (e : term) (x x' : list term),
-    All2 (eval Σ') x x' ->
-    eval Σ' e tBox -> eval Σ' (mkApps e x) tBox.
-Proof.
-  intros Σ' e x H2. 
-  revert e H2; induction x using rev_ind; cbn; intros; eauto.
-  eapply All2_app_inv_l in X as (l1' & l2' & -> & H' & H2).
-  depelim H2.
-  specialize (IHx e _ H' H). simpl.
-  rewrite mkApps_app. simpl. econstructor; eauto.
-Qed.
